@prefix : <http://www.semanticweb.org/owl/owlapi/turtle#> .
@prefix dct: <http://purl.org/dc/terms/> .
@prefix owl: <http://www.w3.org/2002/07/owl#> .
@prefix rdf: <http://www.w3.org/1999/02/22-rdf-syntax-ns#> .
@prefix xml: <http://www.w3.org/XML/1998/namespace> .
@prefix xsd: <http://www.w3.org/2001/XMLSchema#> .
@prefix dcat: <http://www.w3.org/ns/dcat#> .
@prefix foaf: <http://xmlns.com/foaf/0.1/> .
@prefix odrl: <http://www.w3.org/ns/odrl/2/> .
@prefix prov: <http://www.w3.org/ns/prov#> .
@prefix rdfs: <http://www.w3.org/2000/01/rdf-schema#> .
@prefix skos: <http://www.w3.org/2004/02/skos/core#> .
@prefix spdx: <http://spdx.org/rdf/terms/#> .
@prefix vann: <http://purl.org/vocab/vann/> .
@prefix void: <http://rdfs.org/ns/void#> .
@prefix wsdl: <http://www.w3.org/ns/wsdl-rdf#> .
@prefix litre: <http://www.essepuntato.it/2010/06/literalreification/> .
@prefix lvont: <http://lexvo.org/ontology#> .
@prefix dataid: <http://dataid.dbpedia.org/ns/core#> .
@prefix datacite: <http://purl.org/spar/datacite/> .
@base <http://dataid.dbpedia.org/ns/core#> .

<http://dataid.dbpedia.org/ns/core#> rdf:type owl:Ontology ;
                                     
                                     rdfs:label "DataID"@en ;
                                     
                                     vann:preferredNamespacePrefix "dataid"^^xsd:string ;
                                     
                                     vann:preferredNamespaceUri "http://dataid.dbpedia.org/ns/core#" ;
                                     
                                     owl:versionInfo "1.0.0" ;
                                     
                                     rdfs:comment "DBpedia Data ID is an ontology with the goal of extensively describing datasets via RDF files in a uniform way. Established vocabularies like DCAT, VoID, Prov-O are used for maximum compatibility."@en ;
                                     
                                     owl:imports rdfs: ,
                                                 <http://www.w3.org/ns/dcat> ,
                                                 <http://www.w3.org/ns/prov-o-20130430> ,
                                                 foaf: .


#################################################################
#
#    Annotation properties
#
#################################################################


###  http://purl.org/dc/elements/1.1/contributor

<http://purl.org/dc/elements/1.1/contributor> rdf:type owl:AnnotationProperty .



###  http://purl.org/dc/elements/1.1/coverage

<http://purl.org/dc/elements/1.1/coverage> rdf:type owl:AnnotationProperty .



###  http://purl.org/dc/elements/1.1/creator

<http://purl.org/dc/elements/1.1/creator> rdf:type owl:AnnotationProperty .



###  http://purl.org/dc/elements/1.1/date

<http://purl.org/dc/elements/1.1/date> rdf:type owl:AnnotationProperty .



###  http://purl.org/dc/elements/1.1/description

<http://purl.org/dc/elements/1.1/description> rdf:type owl:AnnotationProperty .



###  http://purl.org/dc/elements/1.1/format

<http://purl.org/dc/elements/1.1/format> rdf:type owl:AnnotationProperty .



###  http://purl.org/dc/elements/1.1/identifier

<http://purl.org/dc/elements/1.1/identifier> rdf:type owl:AnnotationProperty .



###  http://purl.org/dc/elements/1.1/language

<http://purl.org/dc/elements/1.1/language> rdf:type owl:AnnotationProperty .



###  http://purl.org/dc/elements/1.1/publisher

<http://purl.org/dc/elements/1.1/publisher> rdf:type owl:AnnotationProperty .



###  http://purl.org/dc/elements/1.1/relation

<http://purl.org/dc/elements/1.1/relation> rdf:type owl:AnnotationProperty .



###  http://purl.org/dc/elements/1.1/rights

<http://purl.org/dc/elements/1.1/rights> rdf:type owl:AnnotationProperty .



###  http://purl.org/dc/elements/1.1/source

<http://purl.org/dc/elements/1.1/source> rdf:type owl:AnnotationProperty .



###  http://purl.org/dc/elements/1.1/subject

<http://purl.org/dc/elements/1.1/subject> rdf:type owl:AnnotationProperty .



###  http://purl.org/dc/elements/1.1/title

<http://purl.org/dc/elements/1.1/title> rdf:type owl:AnnotationProperty .



###  http://purl.org/dc/elements/1.1/type

<http://purl.org/dc/elements/1.1/type> rdf:type owl:AnnotationProperty .



###  http://purl.org/dc/terms/abstract

dct:abstract rdf:type owl:AnnotationProperty ;
             
             rdfs:label "Abstract"@en ;
             
             rdfs:comment "A summary of the resource."@en ;
             
             dct:hasVersion <http://dublincore.org/usage/terms/history/#abstract-003> ;
             
             rdfs:subPropertyOf <http://purl.org/dc/elements/1.1/description> ;
             
             rdfs:isDefinedBy dct: ;
             
             rdfs:subPropertyOf dct:description .



###  http://purl.org/dc/terms/accessRights

dct:accessRights rdf:type owl:AnnotationProperty ;
                 
                 rdfs:label "Access Rights"@en ;
                 
                 dct:description "Access Rights may include information regarding access or restrictions based on privacy, security, or other policies."@en ;
                 
                 rdfs:comment "Information about who can access the resource or an indication of its security status."@en ;
                 
                 dct:hasVersion <http://dublincore.org/usage/terms/history/#accessRights-002> ;
                 
                 rdfs:subPropertyOf <http://purl.org/dc/elements/1.1/rights> ;
                 
                 rdfs:isDefinedBy dct: .



###  http://purl.org/dc/terms/alternative

dct:alternative rdf:type owl:AnnotationProperty ;
                
                rdfs:label "Alternative Title"@en ;
                
                rdfs:comment "An alternative name for the resource."@en ;
                
                dct:description "The distinction between titles and alternative titles is application-specific."@en ;
                
                dct:hasVersion <http://dublincore.org/usage/terms/history/#alternative-003> ;
                
                rdfs:subPropertyOf <http://purl.org/dc/elements/1.1/title> ;
                
                rdfs:isDefinedBy dct: .



###  http://purl.org/dc/terms/available

dct:available rdf:type owl:AnnotationProperty ;
              
              rdfs:label "Date Available"@en ;
              
              rdfs:comment "Date (often a range) that the resource became or will become available."@en ;
              
              dct:hasVersion <http://dublincore.org/usage/terms/history/#available-003> ;
              
              rdfs:subPropertyOf <http://purl.org/dc/elements/1.1/date> ;
              
              rdfs:isDefinedBy dct: .



###  http://purl.org/dc/terms/bibliographicCitation

dct:bibliographicCitation rdf:type owl:AnnotationProperty ;
                          
                          rdfs:label "Bibliographic Citation"@en ;
                          
                          rdfs:comment "A bibliographic reference for the resource."@en ;
                          
                          dct:description "Recommended practice is to include sufficient bibliographic detail to identify the resource as unambiguously as possible."@en ;
                          
                          dct:hasVersion <http://dublincore.org/usage/terms/history/#bibliographicCitation-002> ;
                          
                          rdfs:subPropertyOf <http://purl.org/dc/elements/1.1/identifier> ;
                          
                          rdfs:isDefinedBy dct: .



###  http://purl.org/dc/terms/conformsTo

dct:conformsTo rdf:type owl:AnnotationProperty ;
               
               rdfs:label "Conforms To"@en ;
               
               rdfs:comment "An established standard to which the described resource conforms."@en ;
               
               dct:hasVersion <http://dublincore.org/usage/terms/history/#conformsTo-003> ;
               
               rdfs:subPropertyOf <http://purl.org/dc/elements/1.1/relation> ;
               
               rdfs:isDefinedBy dct: ;
               
               rdfs:subPropertyOf dct:relation .



###  http://purl.org/dc/terms/contributor

dct:contributor rdf:type owl:AnnotationProperty ;
                
                rdfs:label "Contributor"@en ;
                
                rdfs:comment "An entity responsible for making contributions to the resource."@en ;
                
                dct:description "Examples of a Contributor include a person, an organization, or a service."@en ;
                
                dct:hasVersion <http://dublincore.org/usage/terms/history/#contributorT-001> ;
                
                rdfs:subPropertyOf <http://purl.org/dc/elements/1.1/contributor> ;
                
                rdfs:isDefinedBy dct: .



###  http://purl.org/dc/terms/coverage

dct:coverage rdf:type owl:AnnotationProperty ;
             
             rdfs:label "Coverage"@en ;
             
             dct:description "Spatial topic and spatial applicability may be a named place or a location specified by its geographic coordinates. Temporal topic may be a named period, date, or date range. A jurisdiction may be a named administrative entity or a geographic place to which the resource applies. Recommended best practice is to use a controlled vocabulary such as the Thesaurus of Geographic Names [TGN]. Where appropriate, named places or time periods can be used in preference to numeric identifiers such as sets of coordinates or date ranges."@en ;
             
             rdfs:comment "The spatial or temporal topic of the resource, the spatial applicability of the resource, or the jurisdiction under which the resource is relevant."@en ;
             
             dct:hasVersion <http://dublincore.org/usage/terms/history/#coverageT-001> ;
             
             rdfs:subPropertyOf <http://purl.org/dc/elements/1.1/coverage> ;
             
             rdfs:isDefinedBy dct: .



###  http://purl.org/dc/terms/created

dct:created rdf:type owl:AnnotationProperty ;
            
            rdfs:label "Date Created"@en ;
            
            rdfs:comment "Date of creation of the resource."@en ;
            
            dct:hasVersion <http://dublincore.org/usage/terms/history/#created-003> ;
            
            rdfs:subPropertyOf <http://purl.org/dc/elements/1.1/date> ;
            
            rdfs:isDefinedBy dct: .



###  http://purl.org/dc/terms/creator

dct:creator rdf:type owl:AnnotationProperty ;
            
            rdfs:label "Creator"@en ;
            
            rdfs:comment "An entity primarily responsible for making the resource."@en ;
            
            dct:description "Examples of a Creator include a person, an organization, or a service."@en ;
            
            dct:hasVersion <http://dublincore.org/usage/terms/history/#creatorT-002> ;
            
            rdfs:subPropertyOf <http://purl.org/dc/elements/1.1/creator> ;
            
            rdfs:isDefinedBy dct: .



###  http://purl.org/dc/terms/date

dct:date rdf:type owl:AnnotationProperty ;
         
         rdfs:label "Date"@en ;
         
         rdfs:comment "A point or period of time associated with an event in the lifecycle of the resource."@en ;
         
         dct:description "Date may be used to express temporal information at any level of granularity.  Recommended best practice is to use an encoding scheme, such as the W3CDTF profile of ISO 8601 [W3CDTF]."@en ;
         
         dct:hasVersion <http://dublincore.org/usage/terms/history/#dateT-001> ;
         
         rdfs:subPropertyOf <http://purl.org/dc/elements/1.1/date> ;
         
         rdfs:isDefinedBy dct: .



###  http://purl.org/dc/terms/dateAccepted

dct:dateAccepted rdf:type owl:AnnotationProperty ;
                 
                 rdfs:label "Date Accepted"@en ;
                 
                 rdfs:comment "Date of acceptance of the resource."@en ;
                 
                 dct:description "Examples of resources to which a Date Accepted may be relevant are a thesis (accepted by a university department) or an article (accepted by a journal)."@en ;
                 
                 dct:hasVersion <http://dublincore.org/usage/terms/history/#dateAccepted-002> ;
                 
                 rdfs:subPropertyOf <http://purl.org/dc/elements/1.1/date> ;
                 
                 rdfs:isDefinedBy dct: .



###  http://purl.org/dc/terms/dateCopyrighted

dct:dateCopyrighted rdf:type owl:AnnotationProperty ;
                    
                    rdfs:label "Date Copyrighted"@en ;
                    
                    rdfs:comment "Date of copyright."@en ;
                    
                    dct:hasVersion <http://dublincore.org/usage/terms/history/#dateCopyrighted-002> ;
                    
                    rdfs:subPropertyOf <http://purl.org/dc/elements/1.1/date> ;
                    
                    rdfs:isDefinedBy dct: .



###  http://purl.org/dc/terms/dateSubmitted

dct:dateSubmitted rdf:type owl:AnnotationProperty ;
                  
                  rdfs:label "Date Submitted"@en ;
                  
                  rdfs:comment "Date of submission of the resource."@en ;
                  
                  dct:description "Examples of resources to which a Date Submitted may be relevant are a thesis (submitted to a university department) or an article (submitted to a journal)."@en ;
                  
                  dct:hasVersion <http://dublincore.org/usage/terms/history/#dateSubmitted-002> ;
                  
                  rdfs:subPropertyOf <http://purl.org/dc/elements/1.1/date> ;
                  
                  rdfs:isDefinedBy dct: .



###  http://purl.org/dc/terms/description

dct:description rdf:type owl:AnnotationProperty ;
                
                rdfs:label "Description"@en ;
                
                rdfs:comment "An account of the resource."@en ;
                
                dct:description "Description may include but is not limited to: an abstract, a table of contents, a graphical representation, or a free-text account of the resource."@en ;
                
                dct:hasVersion <http://dublincore.org/usage/terms/history/#descriptionT-001> ;
                
                rdfs:subPropertyOf <http://purl.org/dc/elements/1.1/description> ;
                
                rdfs:isDefinedBy dct: .



###  http://purl.org/dc/terms/extent

dct:extent rdfs:label "Extent"@en ;
           
           rdfs:comment "The size or duration of the resource."@en ;
           
           dct:hasVersion <http://dublincore.org/usage/terms/history/#extent-003> ;
           
           rdfs:subPropertyOf <http://purl.org/dc/elements/1.1/format> ;
           
           rdfs:isDefinedBy dct: .



###  http://purl.org/dc/terms/format

dct:format rdf:type owl:AnnotationProperty ;
           
           rdfs:label "Format"@en ;
           
           dct:description "Examples of dimensions include size and duration. Recommended best practice is to use a controlled vocabulary such as the list of Internet Media Types [MIME]."@en ;
           
           rdfs:comment "The file format, physical medium, or dimensions of the resource."@en ;
           
           dct:hasVersion <http://dublincore.org/usage/terms/history/#formatT-001> ;
           
           rdfs:subPropertyOf <http://purl.org/dc/elements/1.1/format> ;
           
           rdfs:isDefinedBy dct: .



###  http://purl.org/dc/terms/hasFormat

dct:hasFormat rdf:type owl:AnnotationProperty ;
              
              rdfs:label "Has Format"@en ;
              
              rdfs:comment "A related resource that is substantially the same as the pre-existing described resource, but in another format."@en ;
              
              skos:note "This term is intended to be used with non-literal values as defined in the DCMI Abstract Model (http://dublincore.org/documents/abstract-model/).  As of December 2007, the DCMI Usage Board is seeking a way to express this intention with a formal range declaration."@en ;
              
              dct:hasVersion <http://dublincore.org/usage/terms/history/#hasFormat-003> ;
              
              rdfs:subPropertyOf <http://purl.org/dc/elements/1.1/relation> ;
              
              rdfs:isDefinedBy dct: ;
              
              rdfs:subPropertyOf dct:relation .



###  http://purl.org/dc/terms/hasPart

dct:hasPart rdf:type owl:AnnotationProperty ;
            
            rdfs:label "Has Part"@en ;
            
            rdfs:comment "A related resource that is included either physically or logically in the described resource."@en ;
            
            skos:note "This term is intended to be used with non-literal values as defined in the DCMI Abstract Model (http://dublincore.org/documents/abstract-model/).  As of December 2007, the DCMI Usage Board is seeking a way to express this intention with a formal range declaration."@en ;
            
            dct:hasVersion <http://dublincore.org/usage/terms/history/#hasPart-003> ;
            
            rdfs:subPropertyOf <http://purl.org/dc/elements/1.1/relation> ;
            
            rdfs:isDefinedBy dct: ;
            
            rdfs:subPropertyOf dct:relation .



###  http://purl.org/dc/terms/hasVersion

dct:hasVersion rdf:type owl:AnnotationProperty ;
               
               rdfs:label "Has Version"@en ;
               
               rdfs:comment "A related resource that is a version, edition, or adaptation of the described resource."@en ;
               
               skos:note "This term is intended to be used with non-literal values as defined in the DCMI Abstract Model (http://dublincore.org/documents/abstract-model/).  As of December 2007, the DCMI Usage Board is seeking a way to express this intention with a formal range declaration."@en ;
               
               dct:hasVersion <http://dublincore.org/usage/terms/history/#hasVersion-003> ;
               
               rdfs:subPropertyOf <http://purl.org/dc/elements/1.1/relation> ;
               
               rdfs:isDefinedBy dct: ;
               
               rdfs:subPropertyOf dct:relation .



###  http://purl.org/dc/terms/identifier

dct:identifier rdf:type owl:AnnotationProperty ;
               
               rdfs:label "Identifier"@en ;
               
               rdfs:comment "An unambiguous reference to the resource within a given context."@en ;
               
               dct:description "Recommended best practice is to identify the resource by means of a string conforming to a formal identification system. "@en ;
               
               dct:hasVersion <http://dublincore.org/usage/terms/history/#identifierT-001> ;
               
               rdfs:subPropertyOf <http://purl.org/dc/elements/1.1/identifier> ;
               
               rdfs:isDefinedBy dct: .



###  http://purl.org/dc/terms/isFormatOf

dct:isFormatOf rdf:type owl:AnnotationProperty ;
               
               rdfs:label "Is Format Of"@en ;
               
               rdfs:comment "A related resource that is substantially the same as the described resource, but in another format."@en ;
               
               skos:note "This term is intended to be used with non-literal values as defined in the DCMI Abstract Model (http://dublincore.org/documents/abstract-model/).  As of December 2007, the DCMI Usage Board is seeking a way to express this intention with a formal range declaration."@en ;
               
               dct:hasVersion <http://dublincore.org/usage/terms/history/#isFormatOf-003> ;
               
               rdfs:subPropertyOf <http://purl.org/dc/elements/1.1/relation> ;
               
               rdfs:isDefinedBy dct: ;
               
               rdfs:subPropertyOf dct:relation .



###  http://purl.org/dc/terms/isPartOf

dct:isPartOf rdf:type owl:AnnotationProperty ;
             
             rdfs:label "Is Part Of"@en ;
             
             rdfs:comment "A related resource in which the described resource is physically or logically included."@en ;
             
             skos:note "This term is intended to be used with non-literal values as defined in the DCMI Abstract Model (http://dublincore.org/documents/abstract-model/).  As of December 2007, the DCMI Usage Board is seeking a way to express this intention with a formal range declaration."@en ;
             
             dct:hasVersion <http://dublincore.org/usage/terms/history/#isPartOf-003> ;
             
             rdfs:subPropertyOf <http://purl.org/dc/elements/1.1/relation> ;
             
             rdfs:isDefinedBy dct: ;
             
             rdfs:subPropertyOf dct:relation .



###  http://purl.org/dc/terms/isReferencedBy

dct:isReferencedBy rdf:type owl:AnnotationProperty ;
                   
                   rdfs:label "Is Referenced By"@en ;
                   
                   rdfs:comment "A related resource that references, cites, or otherwise points to the described resource."@en ;
                   
                   skos:note "This term is intended to be used with non-literal values as defined in the DCMI Abstract Model (http://dublincore.org/documents/abstract-model/).  As of December 2007, the DCMI Usage Board is seeking a way to express this intention with a formal range declaration."@en ;
                   
                   dct:hasVersion <http://dublincore.org/usage/terms/history/#isReferencedBy-003> ;
                   
                   rdfs:subPropertyOf <http://purl.org/dc/elements/1.1/relation> ;
                   
                   rdfs:isDefinedBy dct: ;
                   
                   rdfs:subPropertyOf dct:relation .



###  http://purl.org/dc/terms/isReplacedBy

dct:isReplacedBy rdf:type owl:AnnotationProperty ;
                 
                 rdfs:label "Is Replaced By"@en ;
                 
                 rdfs:comment "A related resource that supplants, displaces, or supersedes the described resource."@en ;
                 
                 skos:note "This term is intended to be used with non-literal values as defined in the DCMI Abstract Model (http://dublincore.org/documents/abstract-model/).  As of December 2007, the DCMI Usage Board is seeking a way to express this intention with a formal range declaration."@en ;
                 
                 dct:hasVersion <http://dublincore.org/usage/terms/history/#isReplacedBy-003> ;
                 
                 rdfs:subPropertyOf <http://purl.org/dc/elements/1.1/relation> ;
                 
                 rdfs:isDefinedBy dct: ;
                 
                 rdfs:subPropertyOf dct:relation .



###  http://purl.org/dc/terms/isRequiredBy

dct:isRequiredBy rdf:type owl:AnnotationProperty ;
                 
                 rdfs:label "Is Required By"@en ;
                 
                 rdfs:comment "A related resource that requires the described resource to support its function, delivery, or coherence."@en ;
                 
                 skos:note "This term is intended to be used with non-literal values as defined in the DCMI Abstract Model (http://dublincore.org/documents/abstract-model/).  As of December 2007, the DCMI Usage Board is seeking a way to express this intention with a formal range declaration."@en ;
                 
                 dct:hasVersion <http://dublincore.org/usage/terms/history/#isRequiredBy-003> ;
                 
                 rdfs:subPropertyOf <http://purl.org/dc/elements/1.1/relation> ;
                 
                 rdfs:isDefinedBy dct: ;
                 
                 rdfs:subPropertyOf dct:relation .



###  http://purl.org/dc/terms/isVersionOf

dct:isVersionOf rdf:type owl:AnnotationProperty ;
                
                rdfs:label "Is Version Of"@en ;
                
                rdfs:comment "A related resource of which the described resource is a version, edition, or adaptation."@en ;
                
                dct:description "Changes in version imply substantive changes in content rather than differences in format."@en ;
                
                skos:note "This term is intended to be used with non-literal values as defined in the DCMI Abstract Model (http://dublincore.org/documents/abstract-model/).  As of December 2007, the DCMI Usage Board is seeking a way to express this intention with a formal range declaration."@en ;
                
                dct:hasVersion <http://dublincore.org/usage/terms/history/#isVersionOf-003> ;
                
                rdfs:subPropertyOf <http://purl.org/dc/elements/1.1/relation> ;
                
                rdfs:isDefinedBy dct: ;
                
                rdfs:subPropertyOf dct:relation .



###  http://purl.org/dc/terms/issued

dct:issued rdf:type owl:AnnotationProperty ;
           
           rdfs:label "Date Issued"@en ;
           
           rdfs:comment "Date of formal issuance (e.g., publication) of the resource."@en ;
           
           dct:hasVersion <http://dublincore.org/usage/terms/history/#issued-003> ;
           
           rdfs:subPropertyOf <http://purl.org/dc/elements/1.1/date> ;
           
           rdfs:isDefinedBy dct: .



###  http://purl.org/dc/terms/language

dct:language rdf:type owl:AnnotationProperty ;
             
             rdfs:label "Language"@en ;
             
             rdfs:comment "A language of the resource."@en ;
             
             dct:description "Recommended best practice is to use a controlled vocabulary such as RFC 4646 [RFC4646]."@en ;
             
             dct:hasVersion <http://dublincore.org/usage/terms/history/#languageT-001> ;
             
             rdfs:subPropertyOf <http://purl.org/dc/elements/1.1/language> ;
             
             rdfs:isDefinedBy dct: .



###  http://purl.org/dc/terms/license

dct:license rdf:type owl:AnnotationProperty ;
            
            rdfs:label "License"@en ;
            
            rdfs:comment "A legal document giving official permission to do something with the resource."@en ;
            
            dct:hasVersion <http://dublincore.org/usage/terms/history/#license-002> ;
            
            rdfs:subPropertyOf <http://purl.org/dc/elements/1.1/rights> ;
            
            rdfs:isDefinedBy dct: .



###  http://purl.org/dc/terms/medium

dct:medium rdf:type owl:AnnotationProperty ;
           
           rdfs:label "Medium"@en ;
           
           rdfs:comment "The material or physical carrier of the resource."@en ;
           
           dct:hasVersion <http://dublincore.org/usage/terms/history/#medium-003> ;
           
           rdfs:subPropertyOf <http://purl.org/dc/elements/1.1/format> ;
           
           rdfs:isDefinedBy dct: .



###  http://purl.org/dc/terms/modified

dct:modified rdf:type owl:AnnotationProperty ;
             
             rdfs:label "Date Modified"@en ;
             
             rdfs:comment "Date on which the resource was changed."@en ;
             
             dct:hasVersion <http://dublincore.org/usage/terms/history/#modified-003> ;
             
             rdfs:subPropertyOf <http://purl.org/dc/elements/1.1/date> ;
             
             rdfs:isDefinedBy dct: .



###  http://purl.org/dc/terms/publisher

dct:publisher rdf:type owl:AnnotationProperty ;
              
              rdfs:label "Publisher"@en ;
              
              rdfs:comment "An entity responsible for making the resource available."@en ;
              
              dct:description "Examples of a Publisher include a person, an organization, or a service."@en ;
              
              dct:hasVersion <http://dublincore.org/usage/terms/history/#publisherT-001> ;
              
              rdfs:subPropertyOf <http://purl.org/dc/elements/1.1/publisher> ;
              
              rdfs:isDefinedBy dct: .



###  http://purl.org/dc/terms/references

dct:references rdf:type owl:AnnotationProperty ;
               
               rdfs:label "References"@en ;
               
               rdfs:comment "A related resource that is referenced, cited, or otherwise pointed to by the described resource."@en ;
               
               skos:note "This term is intended to be used with non-literal values as defined in the DCMI Abstract Model (http://dublincore.org/documents/abstract-model/).  As of December 2007, the DCMI Usage Board is seeking a way to express this intention with a formal range declaration."@en ;
               
               dct:hasVersion <http://dublincore.org/usage/terms/history/#references-003> ;
               
               rdfs:subPropertyOf <http://purl.org/dc/elements/1.1/relation> ;
               
               rdfs:isDefinedBy dct: ;
               
               rdfs:subPropertyOf dct:relation .



###  http://purl.org/dc/terms/relation

dct:relation rdf:type owl:AnnotationProperty ;
             
             rdfs:label "Relation"@en ;
             
             rdfs:comment "A related resource."@en ;
             
             dct:description "Recommended best practice is to identify the related resource by means of a string conforming to a formal identification system. "@en ;
             
             skos:note "This term is intended to be used with non-literal values as defined in the DCMI Abstract Model (http://dublincore.org/documents/abstract-model/).  As of December 2007, the DCMI Usage Board is seeking a way to express this intention with a formal range declaration."@en ;
             
             dct:hasVersion <http://dublincore.org/usage/terms/history/#relationT-001> ;
             
             rdfs:subPropertyOf <http://purl.org/dc/elements/1.1/relation> ;
             
             rdfs:isDefinedBy dct: .



###  http://purl.org/dc/terms/replaces

dct:replaces rdf:type owl:AnnotationProperty ;
             
             rdfs:label "Replaces"@en ;
             
             rdfs:comment "A related resource that is supplanted, displaced, or superseded by the described resource."@en ;
             
             skos:note "This term is intended to be used with non-literal values as defined in the DCMI Abstract Model (http://dublincore.org/documents/abstract-model/).  As of December 2007, the DCMI Usage Board is seeking a way to express this intention with a formal range declaration."@en ;
             
             dct:hasVersion <http://dublincore.org/usage/terms/history/#replaces-003> ;
             
             rdfs:subPropertyOf <http://purl.org/dc/elements/1.1/relation> ;
             
             rdfs:isDefinedBy dct: ;
             
             rdfs:subPropertyOf dct:relation .



###  http://purl.org/dc/terms/requires

dct:requires rdf:type owl:AnnotationProperty ;
             
             rdfs:label "Requires"@en ;
             
             rdfs:comment "A related resource that is required by the described resource to support its function, delivery, or coherence."@en ;
             
             skos:note "This term is intended to be used with non-literal values as defined in the DCMI Abstract Model (http://dublincore.org/documents/abstract-model/).  As of December 2007, the DCMI Usage Board is seeking a way to express this intention with a formal range declaration."@en ;
             
             dct:hasVersion <http://dublincore.org/usage/terms/history/#requires-003> ;
             
             rdfs:subPropertyOf <http://purl.org/dc/elements/1.1/relation> ;
             
             rdfs:isDefinedBy dct: ;
             
             rdfs:subPropertyOf dct:relation .



###  http://purl.org/dc/terms/rights

dct:rights rdf:type owl:AnnotationProperty ;
           
           rdfs:label "Rights"@en ;
           
           rdfs:comment "Information about rights held in and over the resource."@en ;
           
           dct:description "Typically, rights information includes a statement about various property rights associated with the resource, including intellectual property rights."@en ;
           
           dct:hasVersion <http://dublincore.org/usage/terms/history/#rightsT-001> ;
           
           rdfs:subPropertyOf <http://purl.org/dc/elements/1.1/rights> ;
           
           rdfs:isDefinedBy dct: .



###  http://purl.org/dc/terms/source

dct:source rdf:type owl:AnnotationProperty ;
           
           rdfs:label "Source"@en ;
           
           rdfs:comment "A related resource from which the described resource is derived."@en ;
           
           dct:description "The described resource may be derived from the related resource in whole or in part. Recommended best practice is to identify the related resource by means of a string conforming to a formal identification system."@en ;
           
           skos:note "This term is intended to be used with non-literal values as defined in the DCMI Abstract Model (http://dublincore.org/documents/abstract-model/).  As of December 2007, the DCMI Usage Board is seeking a way to express this intention with a formal range declaration."@en ;
           
           dct:hasVersion <http://dublincore.org/usage/terms/history/#sourceT-001> ;
           
           rdfs:subPropertyOf <http://purl.org/dc/elements/1.1/source> ;
           
           rdfs:isDefinedBy dct: ;
           
           rdfs:subPropertyOf dct:relation .



###  http://purl.org/dc/terms/spatial

dct:spatial rdf:type owl:AnnotationProperty ;
            
            rdfs:label "Spatial Coverage"@en ;
            
            rdfs:comment "Spatial characteristics of the resource."@en ;
            
            dct:hasVersion <http://dublincore.org/usage/terms/history/#spatial-003> ;
            
            rdfs:subPropertyOf <http://purl.org/dc/elements/1.1/coverage> ;
            
            rdfs:isDefinedBy dct: .



###  http://purl.org/dc/terms/subject

dct:subject rdf:type owl:AnnotationProperty ;
            
            rdfs:label "Subject"@en ;
            
            rdfs:comment "The topic of the resource."@en ;
            
            skos:note "This term is intended to be used with non-literal values as defined in the DCMI Abstract Model (http://dublincore.org/documents/abstract-model/).  As of December 2007, the DCMI Usage Board is seeking a way to express this intention with a formal range declaration."@en ;
            
            dct:description "Typically, the subject will be represented using keywords, key phrases, or classification codes. Recommended best practice is to use a controlled vocabulary."@en ;
            
            dct:hasVersion <http://dublincore.org/usage/terms/history/#subjectT-002> ;
            
            rdfs:subPropertyOf <http://purl.org/dc/elements/1.1/subject> ;
            
            rdfs:isDefinedBy dct: .



###  http://purl.org/dc/terms/tableOfContents

dct:tableOfContents rdf:type owl:AnnotationProperty ;
                    
                    rdfs:label "Table Of Contents"@en ;
                    
                    rdfs:comment "A list of subunits of the resource."@en ;
                    
                    dct:hasVersion <http://dublincore.org/usage/terms/history/#tableOfContents-003> ;
                    
                    rdfs:subPropertyOf <http://purl.org/dc/elements/1.1/description> ;
                    
                    rdfs:isDefinedBy dct: ;
                    
                    rdfs:subPropertyOf dct:description .



###  http://purl.org/dc/terms/temporal

dct:temporal rdf:type owl:AnnotationProperty ;
             
             rdfs:label "Temporal Coverage"@en ;
             
             rdfs:comment "Temporal characteristics of the resource."@en ;
             
             dct:hasVersion <http://dublincore.org/usage/terms/history/#temporal-003> ;
             
             rdfs:subPropertyOf <http://purl.org/dc/elements/1.1/coverage> ;
             
             rdfs:isDefinedBy dct: .



###  http://purl.org/dc/terms/title

dct:title rdf:type owl:AnnotationProperty ;
          
          rdfs:label "Title"@en ;
          
          rdfs:comment "A name given to the resource."@en ;
          
          dct:hasVersion <http://dublincore.org/usage/terms/history/#titleT-002> ;
          
          rdfs:subPropertyOf <http://purl.org/dc/elements/1.1/title> ;
          
          rdfs:isDefinedBy dct: .



###  http://purl.org/dc/terms/type

dct:type rdf:type owl:AnnotationProperty ;
         
         rdfs:label "Type"@en ;
         
         dct:description "Recommended best practice is to use a controlled vocabulary such as the DCMI Type Vocabulary [DCMITYPE]. To describe the file format, physical medium, or dimensions of the resource, use the Format element."@en ;
         
         rdfs:comment "The nature or genre of the resource."@en ;
         
         dct:hasVersion <http://dublincore.org/usage/terms/history/#typeT-001> ;
         
         rdfs:subPropertyOf <http://purl.org/dc/elements/1.1/type> ;
         
         rdfs:isDefinedBy dct: .



###  http://purl.org/dc/terms/valid

dct:valid rdf:type owl:AnnotationProperty ;
          
          rdfs:label "Date Valid"@en ;
          
          rdfs:comment "Date (often a range) of validity of a resource."@en ;
          
          dct:hasVersion <http://dublincore.org/usage/terms/history/#valid-003> ;
          
          rdfs:subPropertyOf <http://purl.org/dc/elements/1.1/date> ;
          
          rdfs:isDefinedBy dct: .



###  http://www.w3.org/2004/02/skos/core#note

skos:note rdf:type owl:AnnotationProperty .



###  http://xmlns.com/foaf/0.1/mbox

foaf:mbox rdf:type owl:AnnotationProperty .



###  http://xmlns.com/foaf/0.1/name

foaf:name rdf:type owl:AnnotationProperty .





#################################################################
#
#    Datatypes
#
#################################################################


###  http://purl.org/dc/terms/Box

dct:Box rdf:type rdfs:Datatype ;
        
        rdfs:label "DCMI Box"@en ;
        
        rdfs:comment "The set of regions in space defined by their geographic coordinates according to the DCMI Box Encoding Scheme."@en ;
        
        rdfs:seeAlso <http://dublincore.org/documents/dcmi-box/> ;
        
        dct:hasVersion <http://dublincore.org/usage/terms/history/#Box-003> ;
        
        rdfs:isDefinedBy dct: .



###  http://purl.org/dc/terms/ISO3166

dct:ISO3166 rdf:type rdfs:Datatype ;
            
            rdfs:label "ISO 3166"@en ;
            
            rdfs:comment "The set of codes listed in ISO 3166-1 for the representation of names of countries."@en ;
            
            dct:hasVersion <http://dublincore.org/usage/terms/history/#ISO3166-004> ;
            
            rdfs:isDefinedBy dct: ;
            
            rdfs:seeAlso <http://www.iso.org/iso/en/prods-services/iso3166ma/02iso-3166-code-lists/list-en1.html> .



###  http://purl.org/dc/terms/ISO639-2

dct:ISO639-2 rdf:type rdfs:Datatype ;
             
             rdfs:label "ISO 639-2"@en ;
             
             rdfs:comment "The three-letter alphabetic codes listed in ISO639-2 for the representation of names of languages."@en ;
             
             dct:hasVersion <http://dublincore.org/usage/terms/history/#ISO639-2-003> ;
             
             rdfs:seeAlso <http://lcweb.loc.gov/standards/iso639-2/langhome.html> ;
             
             rdfs:isDefinedBy dct: .



###  http://purl.org/dc/terms/ISO639-3

dct:ISO639-3 rdf:type rdfs:Datatype ;
             
             rdfs:label "ISO 639-3"@en ;
             
             rdfs:comment "The set of three-letter codes listed in ISO 639-3 for the representation of names of languages."@en ;
             
             dct:hasVersion <http://dublincore.org/usage/terms/history/#ISO639-3-001> ;
             
             rdfs:isDefinedBy dct: ;
             
             rdfs:seeAlso <http://www.sil.org/iso639-3/> .



###  http://purl.org/dc/terms/Period

dct:Period rdf:type rdfs:Datatype ;
           
           rdfs:label "DCMI Period"@en ;
           
           rdfs:comment "The set of time intervals defined by their limits according to the DCMI Period Encoding Scheme."@en ;
           
           rdfs:seeAlso <http://dublincore.org/documents/dcmi-period/> ;
           
           dct:hasVersion <http://dublincore.org/usage/terms/history/#Period-003> ;
           
           rdfs:isDefinedBy dct: .



###  http://purl.org/dc/terms/Point

dct:Point rdf:type rdfs:Datatype ;
          
          rdfs:label "DCMI Point"@en ;
          
          rdfs:comment "The set of points in space defined by their geographic coordinates according to the DCMI Point Encoding Scheme."@en ;
          
          rdfs:seeAlso <http://dublincore.org/documents/dcmi-point/> ;
          
          dct:hasVersion <http://dublincore.org/usage/terms/history/#Point-003> ;
          
          rdfs:isDefinedBy dct: .



###  http://purl.org/dc/terms/RFC1766

dct:RFC1766 rdf:type rdfs:Datatype ;
            
            rdfs:label "RFC 1766"@en ;
            
            rdfs:comment "The set of tags, constructed according to RFC 1766, for the identification of languages."@en ;
            
            dct:hasVersion <http://dublincore.org/usage/terms/history/#RFC1766-003> ;
            
            rdfs:isDefinedBy dct: ;
            
            rdfs:seeAlso <http://www.ietf.org/rfc/rfc1766.txt> .



###  http://purl.org/dc/terms/RFC3066

dct:RFC3066 rdf:type rdfs:Datatype ;
            
            rdfs:label "RFC 3066"@en ;
            
            dct:description "RFC 3066 has been obsoleted by RFC 4646."@en ;
            
            rdfs:comment "The set of tags constructed according to RFC 3066 for the identification of languages."@en ;
            
            dct:hasVersion <http://dublincore.org/usage/terms/history/#RFC3066-002> ;
            
            rdfs:isDefinedBy dct: ;
            
            rdfs:seeAlso <http://www.ietf.org/rfc/rfc3066.txt> .



###  http://purl.org/dc/terms/RFC4646

dct:RFC4646 rdf:type rdfs:Datatype ;
            
            rdfs:label "RFC 4646"@en ;
            
            dct:description "RFC 4646 obsoletes RFC 3066."@en ;
            
            rdfs:comment "The set of tags constructed according to RFC 4646 for the identification of languages."@en ;
            
            dct:hasVersion <http://dublincore.org/usage/terms/history/#RFC4646-001> ;
            
            rdfs:isDefinedBy dct: ;
            
            rdfs:seeAlso <http://www.ietf.org/rfc/rfc4646.txt> .



###  http://purl.org/dc/terms/RFC5646

dct:RFC5646 rdf:type rdfs:Datatype ;
            
            rdfs:label "RFC 5646"@en ;
            
            dct:description "RFC 5646 obsoletes RFC 4646."@en ;
            
            rdfs:comment "The set of tags constructed according to RFC 5646 for the identification of languages."@en ;
            
            dct:hasVersion <http://dublincore.org/usage/terms/history/#RFC5646-001> ;
            
            rdfs:isDefinedBy dct: ;
            
            rdfs:seeAlso <http://www.ietf.org/rfc/rfc5646.txt> .



###  http://purl.org/dc/terms/URI

dct:URI rdf:type rdfs:Datatype ;
        
        rdfs:label "URI"@en ;
        
        rdfs:comment "The set of identifiers constructed according to the generic syntax for Uniform Resource Identifiers as specified by the Internet Engineering Task Force."@en ;
        
        dct:hasVersion <http://dublincore.org/usage/terms/history/#URI-003> ;
        
        rdfs:isDefinedBy dct: ;
        
        rdfs:seeAlso <http://www.ietf.org/rfc/rfc3986.txt> .



###  http://purl.org/dc/terms/W3CDTF

dct:W3CDTF rdf:type rdfs:Datatype ;
           
           rdfs:label "W3C-DTF"@en ;
           
           rdfs:comment "The set of dates and times constructed according to the W3C Date and Time Formats Specification."@en ;
           
           dct:hasVersion <http://dublincore.org/usage/terms/history/#W3CDTF-003> ;
           
           rdfs:isDefinedBy dct: ;
           
           rdfs:seeAlso <http://www.w3.org/TR/NOTE-datetime> .



###  http://www.w3.org/2001/XMLSchema#date

xsd:date rdf:type rdfs:Datatype .





#################################################################
#
#    Object Properties
#
#################################################################


###  http://dataid.dbpedia.org/ns/core#accessProcedure

dataid:accessProcedure rdf:type owl:ObjectProperty ;
                       
                       rdfs:label "access procedure"@en ;
                       
                       rdfs:comment "Describes the steps which have to be taken to gain access to the described data at the location of a distribution (e.g. register an account to gain dct:accessRights)."@en ;
                       
                       rdfs:isDefinedBy <http://dataid.dbpedia.org/ns/core#> ;
                       
                       rdfs:domain dataid:Distribution ;
                       
                       rdfs:range rdfs:Literal .



###  http://dataid.dbpedia.org/ns/core#allowsFor

dataid:allowsFor rdf:type owl:ObjectProperty ;
                 
                 rdfs:label "allowes for"@en ;
                 
                 rdfs:comment "AgentRoles allows an agent to execute certain actions."@en ;
                 
                 rdfs:isDefinedBy <http://dataid.dbpedia.org/ns/core#> ;
                 
                 rdfs:domain dataid:AgentRole ;
                 
                 rdfs:range dataid:AuthorizedAction .



###  http://dataid.dbpedia.org/ns/core#associatedAgent

dataid:associatedAgent rdf:type owl:ObjectProperty ;
                       
                       rdfs:label "associated agent"@en ;
                       
                       rdfs:comment "some agent generally connected to the dataset, their function to be specified by their rdf:type"@en ;
                       
                       rdfs:isDefinedBy <http://dataid.dbpedia.org/ns/core#> ;
                       
                       rdfs:range dataid:Agent ;
                       
                       rdfs:domain prov:Entity ;
                       
                       rdfs:subPropertyOf prov:wasAttributedTo ;
                       
                       owl:propertyChainAxiom ( dataid:underAuthorization
                                                dataid:authorizedAgent
                                              ) .



###  http://dataid.dbpedia.org/ns/core#authorityAgentRole

dataid:authorityAgentRole rdf:type owl:ObjectProperty ;
                          
                          rdfs:label "authority agent role"@en ;
                          
                          rdfs:comment "Adds a role an agent can administer in the scope provided by the Authorization, thereby allowing for certain actions an agent can execute."@en ;
                          
                          rdfs:isDefinedBy <http://dataid.dbpedia.org/ns/core#> ;
                          
                          rdfs:range dataid:AgentRole ;
                          
                          rdfs:domain dataid:Authorization ;
                          
                          rdfs:subPropertyOf prov:hadRole .



###  http://dataid.dbpedia.org/ns/core#authorityChain

dataid:authorityChain rdf:type owl:ObjectProperty ,
                               owl:TransitiveProperty ;
                      
                      rdfs:label "authority chain"@en ;
                      
                      rdfs:comment """This property (with its sub-properties) describes how an dataid:Authorization is spread to other entities (lower level entities, like Dataset & Distribution). 
		This inferred chain of authority can be overwritten by introducing other dataid:Authorization objects with the scope of lower level entities. See the example in Github for more information."""@en ;
                      
                      rdfs:isDefinedBy <http://dataid.dbpedia.org/ns/core#> ;
                      
                      rdfs:range prov:Entity ;
                      
                      rdfs:domain prov:Entity .



###  http://dataid.dbpedia.org/ns/core#authoritySubChain1

dataid:authoritySubChain1 rdf:type owl:ObjectProperty ;
                          
                          rdfs:label "dataid to subset authority chain"@en ;
                          
                          rdfs:comment "Represents the authority link between the DataID and Subset entities (if connectd by foaf:primaryTopic/void:subset)."@en ;
                          
                          rdfs:isDefinedBy <http://dataid.dbpedia.org/ns/core#> ;
                          
                          rdfs:subPropertyOf dataid:authorityChain ;
                          
                          owl:propertyChainAxiom ( foaf:primaryTopic
                                                   void:subset
                                                 ) .



###  http://dataid.dbpedia.org/ns/core#authoritySubChain2

dataid:authoritySubChain2 rdf:type owl:ObjectProperty ;
                          
                          rdfs:label "dataid to distribution authority chain"@en ;
                          
                          rdfs:comment "Represents the authority link between the DataID and Distribution entities (if connectd by foaf:primaryTopic/dcat:distribution)."@en ;
                          
                          rdfs:isDefinedBy <http://dataid.dbpedia.org/ns/core#> ;
                          
                          rdfs:subPropertyOf dataid:authorityChain ;
                          
                          owl:propertyChainAxiom ( foaf:primaryTopic
                                                   dcat:distribution
                                                 ) .



###  http://dataid.dbpedia.org/ns/core#authoritySubChain3

dataid:authoritySubChain3 rdf:type owl:ObjectProperty ;
                          
                          rdfs:label "dataset to distribution authority chain"@en ;
                          
                          rdfs:comment "Represents the authority link between a Dataset and Distribution entities (via a scond Dataset)."@en ;
                          
                          rdfs:isDefinedBy <http://dataid.dbpedia.org/ns/core#> ;
                          
                          rdfs:subPropertyOf dataid:authorityChain ;
                          
                          owl:propertyChainAxiom ( void:subset
                                                   dcat:distribution
                                                 ) .



###  http://dataid.dbpedia.org/ns/core#authoritySubChain4

dataid:authoritySubChain4 rdf:type owl:ObjectProperty ;
                          
                          rdfs:label "dataset to dataset to dataset authority chain"@en ;
                          
                          rdfs:comment "Represents the authority link between three Dataset entities (if connectd by void:subset twice)."@en ;
                          
                          rdfs:isDefinedBy <http://dataid.dbpedia.org/ns/core#> ;
                          
                          rdfs:subPropertyOf dataid:authorityChain ;
                          
                          owl:propertyChainAxiom ( void:subset
                                                   void:subset
                                                 ) .



###  http://dataid.dbpedia.org/ns/core#authoritySubChain5

dataid:authoritySubChain5 rdf:type owl:ObjectProperty ;
                          
                          rdfs:label "dataid to distribution authority chain"@en ;
                          
                          rdfs:comment "Represents the authority link between the DataID and Distribution entities (if connectd by foaf:primaryTopic/dcat:distribution)."@en ;
                          
                          rdfs:isDefinedBy <http://dataid.dbpedia.org/ns/core#> ;
                          
                          rdfs:subPropertyOf dataid:authorityChain ;
                          
                          owl:propertyChainAxiom ( foaf:primaryTopic
                                                   void:subset
                                                   dcat:distribution
                                                 ) .



###  http://dataid.dbpedia.org/ns/core#authoritySubChain6

dataid:authoritySubChain6 rdf:type owl:ObjectProperty ;
                          
                          rdfs:label "dataset to distribution authority chain"@en ;
                          
                          rdfs:comment "Represents the authority link between a Dataset and Distribution entities (via a scond Dataset)."@en ;
                          
                          rdfs:isDefinedBy <http://dataid.dbpedia.org/ns/core#> ;
                          
                          rdfs:subPropertyOf dataid:authorityChain ;
                          
                          owl:propertyChainAxiom ( void:subset
                                                   void:subset
                                                   dcat:distribution
                                                 ) .



###  http://dataid.dbpedia.org/ns/core#authoritySubChain7

dataid:authoritySubChain7 rdf:type owl:ObjectProperty ;
                          
                          rdfs:label "dataset to dataset to dataset authority chain"@en ;
                          
                          rdfs:comment "Represents the authority link between three Dataset entities (if connectd by void:subset twice)."@en ;
                          
                          rdfs:isDefinedBy <http://dataid.dbpedia.org/ns/core#> ;
                          
                          rdfs:subPropertyOf dataid:authorityChain ;
                          
                          owl:propertyChainAxiom ( foaf:primaryTopic
                                                   void:subset
                                                   void:subset
                                                 ) .



###  http://dataid.dbpedia.org/ns/core#authorizedAction

dataid:authorizedAction rdf:type owl:ObjectProperty ;
                        
                        rdfs:label "authorized action"@en ;
                        
                        rdfs:comment "Actions, agents are allowed to execute under a given Authorization, without regard to an AgentRole optionally specified in addition."@en ;
                        
                        rdfs:isDefinedBy <http://dataid.dbpedia.org/ns/core#> ;
                        
                        rdfs:domain dataid:Authorization ;
                        
                        rdfs:range dataid:AuthorizedAction ;
                        
                        owl:propertyChainAxiom ( dataid:authorityAgentRole
                                                 dataid:allowsFor
                                               ) .



###  http://dataid.dbpedia.org/ns/core#authorizedAgent

dataid:authorizedAgent rdf:type owl:ObjectProperty ;
                       
                       rdfs:label "authorized agent"@en ;
                       
                       rdfs:comment "Points out the Agent the dataid:Authorization is defined for (e.g. to modify the metadata of a dataset)."@en ;
                       
                       rdfs:isDefinedBy <http://dataid.dbpedia.org/ns/core#> ;
                       
                       rdfs:range dataid:Agent ;
                       
                       rdfs:domain dataid:Authorization ;
                       
                       rdfs:subPropertyOf prov:agent .



###  http://dataid.dbpedia.org/ns/core#authorizedFor

dataid:authorizedFor rdf:type owl:ObjectProperty ;
                     
                     rdfs:label "authorized for"@en ;
                     
                     rdfs:comment "Defines the scope of an dataid:Authorization. An Agent has the right to execute authorized actions in this scope (e.g. a single DataId and all it's datasets)."@en ;
                     
                     rdfs:isDefinedBy <http://dataid.dbpedia.org/ns/core#> ;
                     
                     owl:inverseOf dataid:underAuthorization .



###  http://dataid.dbpedia.org/ns/core#hasAccessLevel

dataid:hasAccessLevel rdf:type owl:FunctionalProperty ,
                               owl:ObjectProperty ;
                      
                      rdfs:label "access level"@en ;
                      
                      rdfs:comment "defines the access rights for DataId related entities"@en ;
                      
                      rdfs:isDefinedBy <http://dataid.dbpedia.org/ns/core#> ;
                      
                      rdfs:range dataid:AccessLevel ;
                      
                      rdfs:domain prov:Entity .



###  http://dataid.dbpedia.org/ns/core#hasAuthorization

dataid:hasAuthorization rdf:type owl:ObjectProperty ;
                        
                        rdfs:label "has authorization"@en ;
                        
                        rdfs:comment "Provides an dataid:Agent with the dataid:Authorization for a given scope of entities (e.g. Dataset, Distribution etc.), to execute certain actions."@en ;
                        
                        rdfs:isDefinedBy <http://dataid.dbpedia.org/ns/core#> ;
                        
                        owl:inverseOf dataid:authorizedAgent .



###  http://dataid.dbpedia.org/ns/core#identifier

dataid:identifier rdf:type owl:InverseFunctionalProperty ,
                           owl:ObjectProperty ;
                  
                  rdfs:label "(additional) identifier"@en ;
                  
                  rdfs:comment "An unique identifier which was created by a SchemaAgency for an agent or entity."@en ;
                  
                  rdfs:isDefinedBy <http://dataid.dbpedia.org/ns/core#> ;
                  
                  rdfs:range dataid:Identifier ;
                  
                  rdfs:subPropertyOf datacite:hasIdentifier ,
                                     foaf:isPrimaryTopicOf .



###  http://dataid.dbpedia.org/ns/core#identifierURL

dataid:identifierURL rdf:type owl:ObjectProperty ;
                     
                     rdfs:label "URL of a page pertaining to this identifier (usualy on a website of the SchemaAgency)."@en ;
                     
                     rdfs:comment "uri/url provided as, or in addition to an id"@en ;
                     
                     rdfs:isDefinedBy <http://dataid.dbpedia.org/ns/core#> ;
                     
                     rdfs:domain dataid:Identifier ;
                     
                     rdfs:range foaf:Document .



###  http://dataid.dbpedia.org/ns/core#innerMediaType

dataid:innerMediaType rdf:type owl:FunctionalProperty ,
                               owl:ObjectProperty ;
                      
                      rdfs:label "inner media type"@en ;
                      
                      rdfs:comment "Points out the MediaType of the (compressed) file inside this one."@en ;
                      
                      rdfs:isDefinedBy <http://dataid.dbpedia.org/ns/core#> ;
                      
                      rdfs:range dataid:MediaType ;
                      
                      rdfs:domain dataid:MediaType ;
                      
                      rdfs:subPropertyOf dcat:mediaType .



###  http://dataid.dbpedia.org/ns/core#isDistributionOf

dataid:isDistributionOf rdf:type owl:ObjectProperty ;
                        
                        rdfs:label "Is distribution of"@en ;
                        
                        rdfs:comment "Inverse property of dcat:distribution, linking a Distribution to a Dataset"@en ;
                        
                        rdfs:isDefinedBy <http://dataid.dbpedia.org/ns/core#> ;
                        
                        rdfs:range dataid:Dataset ;
                        
                        rdfs:domain dataid:Distribution ;
                        
                        owl:inverseOf dcat:distribution .



###  http://dataid.dbpedia.org/ns/core#latestVersion

dataid:latestVersion rdf:type owl:ObjectProperty ;
                     
                     rdfs:label "latest version"@en ;
                     
                     rdfs:comment "Latest version of a DataIdPart"@en ;
                     
                     rdfs:isDefinedBy <http://dataid.dbpedia.org/ns/core#> ;
                     
                     rdfs:range prov:Entity ;
                     
                     rdfs:domain prov:Entity .



###  http://dataid.dbpedia.org/ns/core#nextVersion

dataid:nextVersion rdf:type owl:ObjectProperty ;
                   
                   rdfs:label "next version"@en ;
                   
                   rdfs:comment "Next version of a DataIdPart"@en ;
                   
                   rdfs:isDefinedBy <http://dataid.dbpedia.org/ns/core#> ;
                   
                   rdfs:domain prov:Entity ;
                   
                   rdfs:range prov:Entity .



###  http://dataid.dbpedia.org/ns/core#preview

dataid:preview rdf:type owl:ObjectProperty ;
               
               rdfs:label "data preview"@en ;
               
               rdfs:comment "Provides the uri of a short preview of the data provided by a distribution (do not link to the download or accessURL with this property)."@en ;
               
               rdfs:isDefinedBy <http://dataid.dbpedia.org/ns/core#> ;
               
               rdfs:domain dataid:Distribution ;
               
               rdfs:range foaf:Document .



###  http://dataid.dbpedia.org/ns/core#previousVersion

dataid:previousVersion rdf:type owl:ObjectProperty ;
                       
                       rdfs:label "previous version"@en ;
                       
                       rdfs:comment "previous version of a DataIdPart"@en ;
                       
                       rdfs:isDefinedBy <http://dataid.dbpedia.org/ns/core#> ;
                       
                       rdfs:domain prov:Entity ;
                       
                       rdfs:range prov:Entity .



###  http://dataid.dbpedia.org/ns/core#similarData

dataid:similarData rdf:type owl:ObjectProperty ;
                   
                   rdfs:label "similar data"@en ;
                   
                   rdfs:comment "Points to other dataset containing related data."@en ;
                   
                   rdfs:isDefinedBy <http://dataid.dbpedia.org/ns/core#> ;
                   
                   rdfs:domain dataid:Dataset ;
                   
                   rdfs:subPropertyOf dct:relation ;
                   
                   rdfs:range dcat:Dataset .



###  http://dataid.dbpedia.org/ns/core#softwareRquirement

dataid:softwareRquirement rdf:type owl:ObjectProperty ;
                          
                          rdfs:label "software requirement"@en ;
                          
                          rdfs:comment "software needed to access the data in this distribution"@en ;
                          
                          rdfs:isDefinedBy <http://dataid.dbpedia.org/ns/core#> ;
                          
                          rdfs:domain dataid:Distribution ;
                          
                          rdfs:range foaf:Document .



###  http://dataid.dbpedia.org/ns/core#statement

dataid:statement rdf:type owl:ObjectProperty ;
                 
                 rdfs:label "statement"@en ;
                 
                 rdfs:comment "An actual textual statment"@en ;
                 
                 rdfs:isDefinedBy <http://dataid.dbpedia.org/ns/core#> ;
                 
                 rdfs:domain dataid:SimpleStatement ;
                 
                 rdfs:range rdfs:Literal .



###  http://dataid.dbpedia.org/ns/core#typeExtension

dataid:typeExtension rdf:type owl:ObjectProperty ;
                     
                     rdfs:label "media type file extension"@en ;
                     
                     rdfs:comment "Lists file extensions commonly used with this mime type."@en ;
                     
                     rdfs:isDefinedBy <http://dataid.dbpedia.org/ns/core#> ;
                     
                     rdfs:domain dataid:MediaType ;
                     
                     rdfs:range rdfs:Literal .



###  http://dataid.dbpedia.org/ns/core#typeName

dataid:typeName rdf:type owl:ObjectProperty ;
                
                rdfs:label "media type name"@en ;
                
                rdfs:comment "Names the media types described."@en ;
                
                rdfs:isDefinedBy <http://dataid.dbpedia.org/ns/core#> ;
                
                rdfs:domain dataid:MediaType ;
                
                rdfs:range rdfs:Literal .



###  http://dataid.dbpedia.org/ns/core#typeReference

dataid:typeReference rdf:type owl:ObjectProperty ;
                     
                     rdfs:label "media type reference"@en ;
                     
                     rdfs:comment "Refers to a standard associated with this mime type."@en ;
                     
                     rdfs:isDefinedBy <http://dataid.dbpedia.org/ns/core#> ;
                     
                     rdfs:domain dataid:MediaType ;
                     
                     rdfs:range rdfs:Resource .



###  http://dataid.dbpedia.org/ns/core#typeTemplate

dataid:typeTemplate rdf:type owl:FunctionalProperty ,
                             owl:ObjectProperty ;
                    
                    rdfs:label "media type template"@en ;
                    
                    rdfs:comment "The template (or mime type string) of a media Type."@en ;
                    
                    rdfs:isDefinedBy <http://dataid.dbpedia.org/ns/core#> ;
                    
                    rdfs:domain dataid:MediaType ;
                    
                    rdfs:range rdfs:Literal .



###  http://dataid.dbpedia.org/ns/core#underAuthorization

dataid:underAuthorization rdf:type owl:ObjectProperty ;
                          
                          rdfs:label "under an authorization of"@en ;
                          
                          rdfs:comment "Points out a dataid:Authorization with some degree of authority over this resource."@en ;
                          
                          rdfs:isDefinedBy <http://dataid.dbpedia.org/ns/core#> ;
                          
                          rdfs:range dataid:Authorization ;
                          
                          rdfs:subPropertyOf prov:qualifiedAttribution .



###  http://dataid.dbpedia.org/ns/core#validForAccessLevel

dataid:validForAccessLevel rdf:type owl:ObjectProperty ;
                           
                           rdfs:label "valid for access level"@en ;
                           
                           rdfs:comment "Limits rights and actions an Agent is allowed to take depending on the AccessLevel chosen for this Authorization."@en ;
                           
                           rdfs:isDefinedBy <http://dataid.dbpedia.org/ns/core#> ;
                           
                           rdfs:range dataid:AccessLevel ;
                           
                           rdfs:domain dataid:Authorization .



###  http://dataid.dbpedia.org/ns/core#validFrom

dataid:validFrom rdf:type owl:FunctionalProperty ,
                          owl:ObjectProperty ;
                 
                 rdfs:label "valid from"@en ;
                 
                 rdfs:comment "An Authorization is valid for a specific Agent from a certain point in time."@en ;
                 
                 rdfs:isDefinedBy <http://dataid.dbpedia.org/ns/core#> ;
                 
                 rdfs:domain dataid:Authorization ;
                 
                 rdfs:range xsd:datetime .



###  http://dataid.dbpedia.org/ns/core#validUntil

dataid:validUntil rdf:type owl:FunctionalProperty ,
                           owl:ObjectProperty ;
                  
                  rdfs:label "valid until"@en ;
                  
                  rdfs:comment "An Authorization is valid for a specific Agent until a certain point in time."@en ;
                  
                  rdfs:isDefinedBy <http://dataid.dbpedia.org/ns/core#> ;
                  
                  rdfs:domain dataid:Authorization ;
                  
                  rdfs:range xsd:datetime .



###  http://purl.org/dc/terms/accessRights

dct:accessRights rdf:type owl:ObjectProperty ;
                 
                 rdfs:label "Access Rights"@en ;
                 
                 dct:description "Access Rights may include information regarding access or restrictions based on privacy, security, or other policies."@en ;
                 
                 rdfs:comment "Information about who can access the resource or an indication of its security status."@en ;
                 
                 dct:hasVersion <http://dublincore.org/usage/terms/history/#accessRights-002> ;
                 
                 rdfs:isDefinedBy dct: ;
                 
                 rdfs:range dct:RightsStatement ;
                 
                 rdfs:subPropertyOf dct:rights .



###  http://purl.org/dc/terms/accrualMethod

dct:accrualMethod rdf:type owl:ObjectProperty ;
                  
                  rdfs:label "Accrual Method"@en ;
                  
                  rdfs:comment "The method by which items are added to a collection."@en ;
                  
                  dct:hasVersion <http://dublincore.org/usage/terms/history/#accrualMethod-003> ;
                  
                  rdfs:domain <http://purl.org/dc/dcmitype/Collection> ;
                  
                  rdfs:isDefinedBy dct: ;
                  
                  rdfs:range dct:MethodOfAccrual .



###  http://purl.org/dc/terms/accrualPeriodicity

dct:accrualPeriodicity rdf:type owl:ObjectProperty ;
                       
                       rdfs:label "Accrual Periodicity"@en ;
                       
                       rdfs:comment "The frequency with which items are added to a collection."@en ;
                       
                       dct:hasVersion <http://dublincore.org/usage/terms/history/#accrualPeriodicity-003> ;
                       
                       rdfs:domain <http://purl.org/dc/dcmitype/Collection> ;
                       
                       rdfs:isDefinedBy dct: ;
                       
                       rdfs:range dct:Frequency .



###  http://purl.org/dc/terms/accrualPolicy

dct:accrualPolicy rdf:type owl:ObjectProperty ;
                  
                  rdfs:label "Accrual Policy"@en ;
                  
                  rdfs:comment "The policy governing the addition of items to a collection."@en ;
                  
                  dct:hasVersion <http://dublincore.org/usage/terms/history/#accrualPolicy-003> ;
                  
                  rdfs:domain <http://purl.org/dc/dcmitype/Collection> ;
                  
                  rdfs:isDefinedBy dct: ;
                  
                  rdfs:range dct:Policy .



###  http://purl.org/dc/terms/audience

dct:audience rdf:type owl:ObjectProperty ;
             
             rdfs:label "Audience"@en ;
             
             rdfs:comment "A class of entity for whom the resource is intended or useful."@en ;
             
             dct:hasVersion <http://dublincore.org/usage/terms/history/#audience-003> ;
             
             rdfs:isDefinedBy dct: ;
             
             rdfs:range dct:AgentClass .



###  http://purl.org/dc/terms/conformsTo

dct:conformsTo rdf:type owl:ObjectProperty ;
               
               rdfs:label "Conforms To"@en ;
               
               rdfs:comment "An established standard to which the described resource conforms."@en ;
               
               dct:hasVersion <http://dublincore.org/usage/terms/history/#conformsTo-003> ;
               
               rdfs:isDefinedBy dct: ;
               
               rdfs:range dct:Standard .



###  http://purl.org/dc/terms/contributor

dct:contributor rdf:type owl:ObjectProperty ;
                
                rdfs:label "Contributor"@en ;
                
                rdfs:comment "An entity responsible for making contributions to the resource."@en ;
                
                dct:description "Examples of a Contributor include a person, an organization, or a service."@en ;
                
                dct:hasVersion <http://dublincore.org/usage/terms/history/#contributorT-001> ;
                
                rdfs:isDefinedBy dct: ;
                
                rdfs:range dct:Agent .



###  http://purl.org/dc/terms/coverage

dct:coverage rdf:type owl:ObjectProperty ;
             
             rdfs:label "Coverage"@en ;
             
             dct:description "Spatial topic and spatial applicability may be a named place or a location specified by its geographic coordinates. Temporal topic may be a named period, date, or date range. A jurisdiction may be a named administrative entity or a geographic place to which the resource applies. Recommended best practice is to use a controlled vocabulary such as the Thesaurus of Geographic Names [TGN]. Where appropriate, named places or time periods can be used in preference to numeric identifiers such as sets of coordinates or date ranges."@en ;
             
             rdfs:comment "The spatial or temporal topic of the resource, the spatial applicability of the resource, or the jurisdiction under which the resource is relevant."@en ;
             
             dct:hasVersion <http://dublincore.org/usage/terms/history/#coverageT-001> ;
             
             rdfs:isDefinedBy dct: ;
             
             rdfs:range dct:LocationPeriodOrJurisdiction .



###  http://purl.org/dc/terms/creator

dct:creator rdf:type owl:ObjectProperty ;
            
            rdfs:label "Creator"@en ;
            
            rdfs:comment "An entity primarily responsible for making the resource."@en ;
            
            dct:description "Examples of a Creator include a person, an organization, or a service."@en ;
            
            dct:hasVersion <http://dublincore.org/usage/terms/history/#creatorT-002> ;
            
            rdfs:isDefinedBy dct: ;
            
            rdfs:range dct:Agent ;
            
            rdfs:subPropertyOf dct:contributor .



###  http://purl.org/dc/terms/educationLevel

dct:educationLevel rdf:type owl:ObjectProperty ;
                   
                   rdfs:label "Audience Education Level"@en ;
                   
                   rdfs:comment "A class of entity, defined in terms of progression through an educational or training context, for which the described resource is intended."@en ;
                   
                   dct:hasVersion <http://dublincore.org/usage/terms/history/#educationLevel-002> ;
                   
                   rdfs:isDefinedBy dct: ;
                   
                   rdfs:range dct:AgentClass ;
                   
                   rdfs:subPropertyOf dct:audience .



###  http://purl.org/dc/terms/extent

dct:extent rdf:type owl:ObjectProperty ;
           
           rdfs:label "Extent"@en ;
           
           rdfs:comment "The size or duration of the resource."@en ;
           
           dct:hasVersion <http://dublincore.org/usage/terms/history/#extent-003> ;
           
           rdfs:isDefinedBy dct: ;
           
           rdfs:range dct:SizeOrDuration ;
           
           rdfs:subPropertyOf dct:format .



###  http://purl.org/dc/terms/format

dct:format rdfs:label "Format"@en ;
           
           dct:description "Examples of dimensions include size and duration. Recommended best practice is to use a controlled vocabulary such as the list of Internet Media Types [MIME]."@en ;
           
           rdfs:comment "The file format, physical medium, or dimensions of the resource."@en ;
           
           dct:hasVersion <http://dublincore.org/usage/terms/history/#formatT-001> ;
           
           rdfs:isDefinedBy dct: ;
           
           rdfs:range dct:MediaTypeOrExtent .



###  http://purl.org/dc/terms/instructionalMethod

dct:instructionalMethod rdf:type owl:ObjectProperty ;
                        
                        rdfs:label "Instructional Method"@en ;
                        
                        rdfs:comment "A process, used to engender knowledge, attitudes and skills, that the described resource is designed to support."@en ;
                        
                        dct:description "Instructional Method will typically include ways of presenting instructional materials or conducting instructional activities, patterns of learner-to-learner and learner-to-instructor interactions, and mechanisms by which group and individual levels of learning are measured.  Instructional methods include all aspects of the instruction and learning processes from planning and implementation through evaluation and feedback."@en ;
                        
                        dct:hasVersion <http://dublincore.org/usage/terms/history/#instructionalMethod-002> ;
                        
                        rdfs:isDefinedBy dct: ;
                        
                        rdfs:range dct:MethodOfInstruction .



###  http://purl.org/dc/terms/language

dct:language rdf:type owl:ObjectProperty ;
             
             rdfs:label "Language"@en ;
             
             rdfs:comment "A language of the resource."@en ;
             
             dct:description "Recommended best practice is to use a controlled vocabulary such as RFC 4646 [RFC4646]."@en ;
             
             dct:hasVersion <http://dublincore.org/usage/terms/history/#languageT-001> ;
             
             rdfs:isDefinedBy dct: ;
             
             rdfs:range dct:LinguisticSystem .



###  http://purl.org/dc/terms/license

dct:license rdf:type owl:ObjectProperty ;
            
            rdfs:label "License"@en ;
            
            rdfs:comment "A legal document giving official permission to do something with the resource."@en ;
            
            dct:hasVersion <http://dublincore.org/usage/terms/history/#license-002> ;
            
            rdfs:isDefinedBy dct: ;
            
            rdfs:range dct:LicenseDocument ;
            
            rdfs:subPropertyOf dct:rights .



###  http://purl.org/dc/terms/mediator

dct:mediator rdf:type owl:ObjectProperty ;
             
             rdfs:label "Mediator"@en ;
             
             rdfs:comment "An entity that mediates access to the resource and for whom the resource is intended or useful."@en ;
             
             dct:description "In an educational context, a mediator might be a parent, teacher, teaching assistant, or care-giver."@en ;
             
             dct:hasVersion <http://dublincore.org/usage/terms/history/#mediator-003> ;
             
             rdfs:isDefinedBy dct: ;
             
             rdfs:range dct:AgentClass ;
             
             rdfs:subPropertyOf dct:audience .



###  http://purl.org/dc/terms/medium

dct:medium rdf:type owl:ObjectProperty ;
           
           rdfs:label "Medium"@en ;
           
           rdfs:comment "The material or physical carrier of the resource."@en ;
           
           dct:hasVersion <http://dublincore.org/usage/terms/history/#medium-003> ;
           
           rdfs:isDefinedBy dct: ;
           
           rdfs:range dct:PhysicalMedium ;
           
           rdfs:domain dct:PhysicalResource ;
           
           rdfs:subPropertyOf dct:format .



###  http://purl.org/dc/terms/provenance

dct:provenance rdf:type owl:ObjectProperty ;
               
               rdfs:label "Provenance"@en ;
               
               rdfs:comment "A statement of any changes in ownership and custody of the resource since its creation that are significant for its authenticity, integrity, and interpretation."@en ;
               
               dct:description "The statement may include a description of any changes successive custodians made to the resource."@en ;
               
               dct:hasVersion <http://dublincore.org/usage/terms/history/#provenance-002> ;
               
               rdfs:isDefinedBy dct: ;
               
               rdfs:range dct:ProvenanceStatement .



###  http://purl.org/dc/terms/publisher

dct:publisher rdf:type owl:ObjectProperty ;
              
              rdfs:label "Publisher"@en ;
              
              rdfs:comment "An entity responsible for making the resource available."@en ;
              
              dct:description "Examples of a Publisher include a person, an organization, or a service."@en ;
              
              dct:hasVersion <http://dublincore.org/usage/terms/history/#publisherT-001> ;
              
              rdfs:isDefinedBy dct: ;
              
              rdfs:range dct:Agent .



###  http://purl.org/dc/terms/references

dct:references rdfs:label "References"@en ;
               
               rdfs:comment "A related resource that is referenced, cited, or otherwise pointed to by the described resource."@en ;
               
               skos:note "This term is intended to be used with non-literal values as defined in the DCMI Abstract Model (http://dublincore.org/documents/abstract-model/).  As of December 2007, the DCMI Usage Board is seeking a way to express this intention with a formal range declaration."@en ;
               
               dct:hasVersion <http://dublincore.org/usage/terms/history/#references-003> ;
               
               rdfs:isDefinedBy dct: .



###  http://purl.org/dc/terms/relation

dct:relation rdfs:label "Relation"@en ;
             
             rdfs:comment "A related resource."@en ;
             
             dct:description "Recommended best practice is to identify the related resource by means of a string conforming to a formal identification system. "@en ;
             
             skos:note "This term is intended to be used with non-literal values as defined in the DCMI Abstract Model (http://dublincore.org/documents/abstract-model/).  As of December 2007, the DCMI Usage Board is seeking a way to express this intention with a formal range declaration."@en ;
             
             dct:hasVersion <http://dublincore.org/usage/terms/history/#relationT-001> ;
             
             rdfs:isDefinedBy dct: .



###  http://purl.org/dc/terms/rights

dct:rights rdf:type owl:ObjectProperty ;
           
           rdfs:label "Rights"@en ;
           
           rdfs:comment "Information about rights held in and over the resource."@en ;
           
           dct:description "Typically, rights information includes a statement about various property rights associated with the resource, including intellectual property rights."@en ;
           
           dct:hasVersion <http://dublincore.org/usage/terms/history/#rightsT-001> ;
           
           rdfs:isDefinedBy dct: ;
           
           rdfs:range dct:RightsStatement .



###  http://purl.org/dc/terms/rightsHolder

dct:rightsHolder rdf:type owl:ObjectProperty ;
                 
                 rdfs:label "Rights Holder"@en ;
                 
                 rdfs:comment "A person or organization owning or managing rights over the resource."@en ;
                 
                 dct:hasVersion <http://dublincore.org/usage/terms/history/#rightsHolder-002> ;
                 
                 rdfs:isDefinedBy dct: ;
                 
                 rdfs:range dct:Agent .



###  http://purl.org/dc/terms/spatial

dct:spatial rdf:type owl:ObjectProperty ;
            
            rdfs:label "Spatial Coverage"@en ;
            
            rdfs:comment "Spatial characteristics of the resource."@en ;
            
            dct:hasVersion <http://dublincore.org/usage/terms/history/#spatial-003> ;
            
            rdfs:isDefinedBy dct: ;
            
            rdfs:range dct:Location ;
            
            rdfs:subPropertyOf dct:coverage .



###  http://purl.org/dc/terms/temporal

dct:temporal rdf:type owl:ObjectProperty ;
             
             rdfs:label "Temporal Coverage"@en ;
             
             rdfs:comment "Temporal characteristics of the resource."@en ;
             
             dct:hasVersion <http://dublincore.org/usage/terms/history/#temporal-003> ;
             
             rdfs:isDefinedBy dct: ;
             
             rdfs:range dct:PeriodOfTime ;
             
             rdfs:subPropertyOf dct:coverage .



###  http://purl.org/dc/terms/type

dct:type rdf:type owl:ObjectProperty ;
         
         rdfs:label "Type"@en ;
         
         dct:description "Recommended best practice is to use a controlled vocabulary such as the DCMI Type Vocabulary [DCMITYPE]. To describe the file format, physical medium, or dimensions of the resource, use the Format element."@en ;
         
         rdfs:comment "The nature or genre of the resource."@en ;
         
         dct:hasVersion <http://dublincore.org/usage/terms/history/#typeT-001> ;
         
         rdfs:isDefinedBy dct: ;
         
         rdfs:range rdfs:Class .



###  http://purl.org/spar/datacite/hasIdentifier

datacite:hasIdentifier rdf:type owl:ObjectProperty .



###  http://rdfs.org/ns/void#subset

void:subset rdf:type owl:ObjectProperty .



###  http://www.w3.org/ns/dcat#checksum

dcat:checksum rdf:type owl:ObjectProperty .



###  http://www.w3.org/ns/dcat#distribution




###  http://xmlns.com/foaf/0.1/isPrimaryTopicOf

foaf:isPrimaryTopicOf rdf:type owl:ObjectProperty .



###  http://xmlns.com/foaf/0.1/primaryTopic

foaf:primaryTopic rdf:type owl:ObjectProperty .





#################################################################
#
#    Data properties
#
#################################################################


###  http://dataid.dbpedia.org/ns/core#accessProcedure

dataid:accessProcedure rdf:type owl:DatatypeProperty ;
                       
                       rdfs:label "access procedure"@en ;
                       
                       rdfs:comment "Describes the steps which have to be taken to gain access to the described data at the location of a distribution (e.g. register an account to gain dct:accessRights)."@en ;
                       
                       rdfs:isDefinedBy <http://dataid.dbpedia.org/ns/core#> .



###  http://dataid.dbpedia.org/ns/core#isInheritable

dataid:isInheritable rdf:type owl:DatatypeProperty ,
                              owl:FunctionalProperty ;
                     
                     rdfs:label "is inheritable"@en ;
                     
                     rdfs:comment "Defines that a dataid:Authorization is also valid for the next version of a DataID (if set to 'true' - which should be the default)."@en ,
                                  "The property of certain dataid:Authorization to be able to be inherited"@en ;
                     
                     rdfs:isDefinedBy <http://dataid.dbpedia.org/ns/core#> ;
                     
                     rdfs:domain dataid:Authorization ;
                     
                     rdfs:range xsd:boolean .



###  http://dataid.dbpedia.org/ns/core#statement

dataid:statement rdf:type owl:DatatypeProperty ;
                 
                 rdfs:label "statement"@en ;
                 
                 rdfs:comment "An actual textual statment"@en ;
                 
                 rdfs:isDefinedBy <http://dataid.dbpedia.org/ns/core#> .



###  http://dataid.dbpedia.org/ns/core#typeExtension

dataid:typeExtension rdf:type owl:DatatypeProperty ;
                     
                     rdfs:label "media type file extension"@en ;
                     
                     rdfs:comment "Lists file extensions commonly used with this mime type."@en ;
                     
                     rdfs:isDefinedBy <http://dataid.dbpedia.org/ns/core#> .



###  http://dataid.dbpedia.org/ns/core#typeName

dataid:typeName rdf:type owl:DatatypeProperty ;
                
                rdfs:label "media type name"@en ;
                
                rdfs:comment "Names the media types described."@en ;
                
                rdfs:isDefinedBy <http://dataid.dbpedia.org/ns/core#> .



###  http://dataid.dbpedia.org/ns/core#typeTemplate

dataid:typeTemplate rdf:type owl:DatatypeProperty ,
                             owl:FunctionalProperty ;
                    
                    rdfs:label "media type template"@en ;
                    
                    rdfs:comment "The template (or mime type string) of a media Type."@en ;
                    
                    rdfs:isDefinedBy <http://dataid.dbpedia.org/ns/core#> .



###  http://dataid.dbpedia.org/ns/core#uncompressed

dataid:uncompressed rdf:type owl:DatatypeProperty ;
                    
                    rdfs:label "uncompressed"@en ;
                    
                    rdfs:comment "Records the byte size of the uncompressed version of this file."@en ;
                    
                    rdfs:isDefinedBy <http://dataid.dbpedia.org/ns/core#> ;
                    
                    rdfs:domain dataid:Distribution ;
                    
                    rdfs:range xsd:integer ;
                    
                    rdfs:subPropertyOf dcat:byteSize .



###  http://dataid.dbpedia.org/ns/core#validFrom

dataid:validFrom rdf:type owl:DatatypeProperty ,
                          owl:FunctionalProperty ;
                 
                 rdfs:label "valid from"@en ;
                 
                 rdfs:comment "An Authorization is valid for a specific Agent from a certain point in time."@en ;
                 
                 rdfs:isDefinedBy <http://dataid.dbpedia.org/ns/core#> .



###  http://dataid.dbpedia.org/ns/core#validUntil

dataid:validUntil rdf:type owl:DatatypeProperty ,
                           owl:FunctionalProperty ;
                  
                  rdfs:label "valid until"@en ;
                  
                  rdfs:comment "An Authorization is valid for a specific Agent until a certain point in time."@en ;
                  
                  rdfs:isDefinedBy <http://dataid.dbpedia.org/ns/core#> .



###  http://purl.org/dc/terms/alternative

dct:alternative rdf:type owl:DatatypeProperty ;
                
                rdfs:label "Alternative Title"@en ;
                
                rdfs:comment "An alternative name for the resource."@en ;
                
                dct:description "The distinction between titles and alternative titles is application-specific."@en ;
                
                dct:hasVersion <http://dublincore.org/usage/terms/history/#alternative-003> ;
                
                rdfs:isDefinedBy dct: ;
                
                rdfs:subPropertyOf dct:title ;
                
                rdfs:range rdfs:Literal .



###  http://purl.org/dc/terms/available

dct:available rdf:type owl:DatatypeProperty ;
              
              rdfs:label "Date Available"@en ;
              
              rdfs:comment "Date (often a range) that the resource became or will become available."@en ;
              
              dct:hasVersion <http://dublincore.org/usage/terms/history/#available-003> ;
              
              rdfs:isDefinedBy dct: ;
              
              rdfs:subPropertyOf dct:date ;
              
              rdfs:range rdfs:Literal .



###  http://purl.org/dc/terms/bibliographicCitation

dct:bibliographicCitation rdf:type owl:DatatypeProperty ;
                          
                          rdfs:label "Bibliographic Citation"@en ;
                          
                          rdfs:comment "A bibliographic reference for the resource."@en ;
                          
                          dct:description "Recommended practice is to include sufficient bibliographic detail to identify the resource as unambiguously as possible."@en ;
                          
                          dct:hasVersion <http://dublincore.org/usage/terms/history/#bibliographicCitation-002> ;
                          
                          rdfs:isDefinedBy dct: ;
                          
                          rdfs:domain dct:BibliographicResource ;
                          
                          rdfs:subPropertyOf dct:identifier ;
                          
                          rdfs:range rdfs:Literal .



###  http://purl.org/dc/terms/created

dct:created rdf:type owl:DatatypeProperty ;
            
            rdfs:label "Date Created"@en ;
            
            rdfs:comment "Date of creation of the resource."@en ;
            
            dct:hasVersion <http://dublincore.org/usage/terms/history/#created-003> ;
            
            rdfs:isDefinedBy dct: ;
            
            rdfs:subPropertyOf dct:date ;
            
            rdfs:range rdfs:Literal .



###  http://purl.org/dc/terms/date

dct:date rdf:type owl:DatatypeProperty ;
         
         rdfs:label "Date"@en ;
         
         rdfs:comment "A point or period of time associated with an event in the lifecycle of the resource."@en ;
         
         dct:description "Date may be used to express temporal information at any level of granularity.  Recommended best practice is to use an encoding scheme, such as the W3CDTF profile of ISO 8601 [W3CDTF]."@en ;
         
         dct:hasVersion <http://dublincore.org/usage/terms/history/#dateT-001> ;
         
         rdfs:isDefinedBy dct: ;
         
         rdfs:range rdfs:Literal .



###  http://purl.org/dc/terms/dateAccepted

dct:dateAccepted rdf:type owl:DatatypeProperty ;
                 
                 rdfs:label "Date Accepted"@en ;
                 
                 rdfs:comment "Date of acceptance of the resource."@en ;
                 
                 dct:description "Examples of resources to which a Date Accepted may be relevant are a thesis (accepted by a university department) or an article (accepted by a journal)."@en ;
                 
                 dct:hasVersion <http://dublincore.org/usage/terms/history/#dateAccepted-002> ;
                 
                 rdfs:isDefinedBy dct: ;
                 
                 rdfs:subPropertyOf dct:date ;
                 
                 rdfs:range rdfs:Literal .



###  http://purl.org/dc/terms/dateCopyrighted

dct:dateCopyrighted rdf:type owl:DatatypeProperty ;
                    
                    rdfs:label "Date Copyrighted"@en ;
                    
                    rdfs:comment "Date of copyright."@en ;
                    
                    dct:hasVersion <http://dublincore.org/usage/terms/history/#dateCopyrighted-002> ;
                    
                    rdfs:isDefinedBy dct: ;
                    
                    rdfs:subPropertyOf dct:date ;
                    
                    rdfs:range rdfs:Literal .



###  http://purl.org/dc/terms/dateSubmitted

dct:dateSubmitted rdf:type owl:DatatypeProperty ;
                  
                  rdfs:label "Date Submitted"@en ;
                  
                  rdfs:comment "Date of submission of the resource."@en ;
                  
                  dct:description "Examples of resources to which a Date Submitted may be relevant are a thesis (submitted to a university department) or an article (submitted to a journal)."@en ;
                  
                  dct:hasVersion <http://dublincore.org/usage/terms/history/#dateSubmitted-002> ;
                  
                  rdfs:isDefinedBy dct: ;
                  
                  rdfs:subPropertyOf dct:date ;
                  
                  rdfs:range rdfs:Literal .



###  http://purl.org/dc/terms/identifier

dct:identifier rdf:type owl:DatatypeProperty ;
               
               rdfs:label "Identifier"@en ;
               
               rdfs:comment "An unambiguous reference to the resource within a given context."@en ;
               
               dct:description "Recommended best practice is to identify the resource by means of a string conforming to a formal identification system. "@en ;
               
               dct:hasVersion <http://dublincore.org/usage/terms/history/#identifierT-001> ;
               
               rdfs:isDefinedBy dct: ;
               
               rdfs:range rdfs:Literal .



###  http://purl.org/dc/terms/issued

dct:issued rdf:type owl:DatatypeProperty ;
           
           rdfs:label "Date Issued"@en ;
           
           rdfs:comment "Date of formal issuance (e.g., publication) of the resource."@en ;
           
           dct:hasVersion <http://dublincore.org/usage/terms/history/#issued-003> ;
           
           rdfs:isDefinedBy dct: ;
           
           rdfs:subPropertyOf dct:date ;
           
           rdfs:range rdfs:Literal .



###  http://purl.org/dc/terms/modified

dct:modified rdf:type owl:DatatypeProperty ;
             
             rdfs:label "Date Modified"@en ;
             
             rdfs:comment "Date on which the resource was changed."@en ;
             
             dct:hasVersion <http://dublincore.org/usage/terms/history/#modified-003> ;
             
             rdfs:isDefinedBy dct: ;
             
             rdfs:subPropertyOf dct:date ;
             
             rdfs:range rdfs:Literal .



###  http://purl.org/dc/terms/title

dct:title rdf:type owl:DatatypeProperty ;
          
          rdfs:label "Title"@en ;
          
          rdfs:comment "A name given to the resource."@en ;
          
          dct:hasVersion <http://dublincore.org/usage/terms/history/#titleT-002> ;
          
          rdfs:isDefinedBy dct: ;
          
          rdfs:range rdfs:Literal .



###  http://purl.org/dc/terms/valid

dct:valid rdf:type owl:DatatypeProperty ;
          
          rdfs:label "Date Valid"@en ;
          
          rdfs:comment "Date (often a range) of validity of a resource."@en ;
          
          dct:hasVersion <http://dublincore.org/usage/terms/history/#valid-003> ;
          
          rdfs:isDefinedBy dct: ;
          
          rdfs:subPropertyOf dct:date ;
          
          rdfs:range rdfs:Literal .





#################################################################
#
#    Classes
#
#################################################################


###  http://dataid.dbpedia.org/ns/core#AccessLevel

dataid:AccessLevel rdf:type owl:Class ;
                   
                   rdfs:label "Access level"@en ;
                   
                   rdfs:comment "The level of openness of access to a particular groups of agents"@en ;
                   
                   rdfs:isDefinedBy <http://dataid.dbpedia.org/ns/core#> .



###  http://dataid.dbpedia.org/ns/core#Agent

dataid:Agent rdf:type owl:Class ;
             
             rdfs:label "Agent"@en ;
             
             rdfs:subClassOf dct:Agent ,
                             prov:Agent ,
                             foaf:Agent ;
             
             rdfs:comment "Any type of agent without a specific function."@en ;
             
             rdfs:isDefinedBy <http://dataid.dbpedia.org/ns/core#> .



###  http://dataid.dbpedia.org/ns/core#AgentRole

dataid:AgentRole rdf:type owl:Class ;
                 
                 rdfs:label "Agent role"@en ;
                 
                 rdfs:subClassOf prov:Role ;
                 
                 rdfs:comment "Instances of this class define an array of rights and responsibilities an agent, assigned with this role for a given scope of entities, has to address or can execute."@en ;
                 
                 rdfs:isDefinedBy <http://dataid.dbpedia.org/ns/core#> .



###  http://dataid.dbpedia.org/ns/core#Authorization

dataid:Authorization rdf:type owl:Class ;
                     
                     rdfs:label "Authorization"@en ;
                     
                     rdfs:subClassOf prov:Attribution ;
                     
                     rdfs:comment "This concept defines a scope of Entities and links it to an Agent who has certain rights for those entities (defined by the AgentRole/AuthorizedAction). The scope consists of all Entities directly linked to the dataid:Authorization, as well as transitively dependent Entities."@en ;
                     
                     rdfs:isDefinedBy <http://dataid.dbpedia.org/ns/core#> .



###  http://dataid.dbpedia.org/ns/core#AuthorizedAction

dataid:AuthorizedAction rdf:type owl:Class ;
                        
                        rdfs:label "Authorized action"@en ;
                        
                        rdfs:subClassOf prov:Activity ;
                        
                        rdfs:comment "AgentRoles provide agents with the ability to execute certain actions as well as demand certain responsibilities, which are defines by the instances of this concept."@en ;
                        
                        rdfs:isDefinedBy <http://dataid.dbpedia.org/ns/core#> .



###  http://dataid.dbpedia.org/ns/core#DataId

dataid:DataId rdf:type owl:Class ;
              
              rdfs:label "DataId"@en ;
              
              rdfs:subClassOf void:DatasetDescription ,
                              dcat:CatalogRecord ,
                              prov:Entity ,
                              [ rdf:type owl:Restriction ;
                                owl:onProperty dataid:previousVersion ;
                                owl:allValuesFrom dataid:DataId
                              ] ,
                              [ rdf:type owl:Restriction ;
                                owl:onProperty dataid:nextVersion ;
                                owl:allValuesFrom dataid:DataId
                              ] ,
                              [ rdf:type owl:Restriction ;
                                owl:onProperty dct:language ;
                                owl:allValuesFrom lvont:Language
                              ] ,
                              [ rdf:type owl:Restriction ;
                                owl:onProperty dataid:latestVersion ;
                                owl:allValuesFrom dataid:DataId
                              ] ;
              
              rdfs:comment "A description of one or more datasets. Acts as a dcat:CatalogRecord / void:DatasetDescription."@en ;
              
              dct:description """DataID is a multi-layerd meta-data system, which, in its core, describes datasets and their different manifestations, 
		as well as relations to agents like persons or organisations, in regard to their rights and responsibilities. 
		Depending on context, type of data and use-case, this core ontology can be augmented by multiple existing extensions 
		(e.g. Linked Data, repository descriptions etc.). By describing datasets including content, authors, licenses and provenance via RDF,
		thereby making data accessible to others, is the basic idea of Linked Open Data and is your contribution to a universal data give and take.
		To create DataIDs alongside datasets is the best way of announcing a new dataset and its updates to a global community by placing 
		it in the LOD cloud. You can create your own DataID files for any type of data at http://dataid.dbpedia.org.
		Validating and delivering metadata files in a uniform way, as well as providing the ability to query for datasets, 
		are main objectives of the DBpedia/DataID project."""@en ;
              
              rdfs:isDefinedBy <http://dataid.dbpedia.org/ns/core#> .



###  http://dataid.dbpedia.org/ns/core#Dataset

dataid:Dataset rdf:type owl:Class ;
               
               rdfs:label "Dataset"@en ;
               
               rdfs:subClassOf void:Dataset ,
                               dcat:Dataset ,
                               prov:Entity ,
                               [ rdf:type owl:Restriction ;
                                 owl:onProperty dataid:nextVersion ;
                                 owl:allValuesFrom dataid:Dataset
                               ] ,
                               [ rdf:type owl:Restriction ;
                                 owl:onProperty dataid:previousVersion ;
                                 owl:allValuesFrom dataid:Dataset
                               ] ,
                               [ rdf:type owl:Restriction ;
                                 owl:onProperty void:subset ;
                                 owl:allValuesFrom dataid:Dataset
                               ] ,
                               [ rdf:type owl:Restriction ;
                                 owl:onProperty dct:language ;
                                 owl:allValuesFrom lvont:Language
                               ] ,
                               [ rdf:type owl:Restriction ;
                                 owl:onProperty dataid:latestVersion ;
                                 owl:allValuesFrom dataid:Dataset
                               ] ,
                               [ rdf:type owl:Restriction ;
                                 owl:onProperty dcat:distribution ;
                                 owl:allValuesFrom dataid:Distribution
                               ] ;
               
               rdfs:comment """A collection of data, available for access in one or more formats. Dataset resources describe the concept of the dataset, not it's manifestation (the data itself), which can be acquired as Distribution.
    Datasets are prov:Entities and can be generated by prov:Activities."""@en ;
               
               rdfs:isDefinedBy <http://dataid.dbpedia.org/ns/core#> .



###  http://dataid.dbpedia.org/ns/core#Directory

dataid:Directory rdf:type owl:Class ;
                 
                 rdfs:label "dataset files in one directory"@en ;
                 
                 rdfs:subClassOf dataid:Distribution ;
                 
                 rdfs:comment "A dedicated directory holding multiple files of the same dataset."@en ;
                 
                 rdfs:isDefinedBy <http://dataid.dbpedia.org/ns/core#> .



###  http://dataid.dbpedia.org/ns/core#Distribution

dataid:Distribution rdf:type owl:Class ;
                    
                    rdfs:label "Distribution"@en ;
                    
                    rdfs:subClassOf dcat:Distribution ,
                                    prov:Entity ,
                                    [ rdf:type owl:Restriction ;
                                      owl:onProperty dcat:checksum ;
                                      owl:allValuesFrom spdx:Checksum
                                    ] ,
                                    [ rdf:type owl:Restriction ;
                                      owl:onProperty dataid:latestVersion ;
                                      owl:allValuesFrom dataid:Distribution
                                    ] ,
                                    [ rdf:type owl:Restriction ;
                                      owl:onProperty dct:language ;
                                      owl:allValuesFrom lvont:Language
                                    ] ,
                                    [ rdf:type owl:Restriction ;
                                      owl:onProperty dataid:previousVersion ;
                                      owl:allValuesFrom dataid:Distribution
                                    ] ,
                                    [ rdf:type owl:Restriction ;
                                      owl:onProperty dataid:nextVersion ;
                                      owl:allValuesFrom dataid:Distribution
                                    ] ;
                    
                    rdfs:comment "A way to access a dataset, like a dump file, an endpoint, an API etc."@en ;
                    
                    rdfs:isDefinedBy <http://dataid.dbpedia.org/ns/core#> .



###  http://dataid.dbpedia.org/ns/core#EntitledAction

dataid:EntitledAction rdf:type owl:Class ;
                      
                      rdfs:label "Entitled action"@en ;
                      
                      rdfs:subClassOf dataid:AuthorizedAction ;
                      
                      owl:disjointWith dataid:ResponsibleAction ;
                      
                      rdfs:comment "AgentRoles provide access and modification rights to an agent. Entitled actions should comprise actions pertaining to access/modification restrictions."@en ;
                      
                      rdfs:isDefinedBy <http://dataid.dbpedia.org/ns/core#> .



###  http://dataid.dbpedia.org/ns/core#FileCollection

dataid:FileCollection rdf:type owl:Class ;
                      
                      rdfs:label "dataset files in differnt paths of a distribution"@en ;
                      
                      rdfs:subClassOf dataid:Distribution ;
                      
                      rdfs:comment "Multiple files of a distribution constituting one dataset."@en ;
                      
                      rdfs:isDefinedBy <http://dataid.dbpedia.org/ns/core#> .



###  http://dataid.dbpedia.org/ns/core#Identifier

dataid:Identifier rdf:type owl:Class ;
                  
                  rdfs:label "identifier"@en ;
                  
                  rdfs:subClassOf datacite:Identifier ;
                  
                  rdfs:comment "Uniquly identifies any resource, given an identifier as literal and a correspondng aid/pid scheme (ORCID, ResearcherID etc.). "@en ;
                  
                  rdfs:isDefinedBy <http://dataid.dbpedia.org/ns/core#> .



###  http://dataid.dbpedia.org/ns/core#MediaType

dataid:MediaType rdf:type owl:Class ;
                 
                 rdfs:label "Iana Media Type"@en ;
                 
                 rdfs:subClassOf dct:MediaType ;
                 
                 rdfs:comment "Extends the dct:MediaType class of Dublin Core by implementing the Iana media type description and adding a pointer to inner media types to deal with (multiple) compressions of a serialized file."@en ;
                 
                 rdfs:isDefinedBy <http://dataid.dbpedia.org/ns/core#> .



###  http://dataid.dbpedia.org/ns/core#ResponsibleAction

dataid:ResponsibleAction rdf:type owl:Class ;
                         
                         rdfs:label "responsible actions"@en ;
                         
                         rdfs:subClassOf dataid:AuthorizedAction ;
                         
                         rdfs:comment "AgentRoles provide access rights as well as responsibilities an agent has to attend to in order to fullfill this role. Responsible actions should describe actions pertaining to responsibilities an agent is supposed to do."@en ;
                         
                         rdfs:isDefinedBy <http://dataid.dbpedia.org/ns/core#> .



###  http://dataid.dbpedia.org/ns/core#ServiceEndpoint

dataid:ServiceEndpoint rdf:type owl:Class ;
                       
                       rdfs:label "Service Endpoint"@en ;
                       
                       rdfs:subClassOf dataid:Distribution ,
                                       wsdl:Service ;
                       
                       rdfs:comment "A specific distribution, which is accessible via an access url and provides data as a web service in a certain format."@en ;
                       
                       rdfs:isDefinedBy <http://dataid.dbpedia.org/ns/core#> .



###  http://dataid.dbpedia.org/ns/core#SimpleStatement

dataid:SimpleStatement rdf:type owl:Class ;
                       
                       rdfs:label "Simple Statement"@en ;
                       
                       rdfs:subClassOf dct:ProvenanceStatement ,
                                       dct:RightsStatement ,
                                       dct:Standard ,
                                       [ rdf:type owl:Restriction ;
                                         owl:onProperty dct:references ;
                                         owl:allValuesFrom foaf:Document
                                       ] ;
                       
                       rdfs:comment "Implements the Statement and Standard classes of Dublin Core, containing a textual statement and a reference pointer."@en ;
                       
                       rdfs:isDefinedBy <http://dataid.dbpedia.org/ns/core#> .



###  http://dataid.dbpedia.org/ns/core#SingleFile

dataid:SingleFile rdf:type owl:Class ;
                  
                  rdfs:label "single dump file"@en ;
                  
                  rdfs:subClassOf dataid:Distribution ;
                  
                  rdfs:comment "A single data dump file representing your dataset."@en ;
                  
                  rdfs:isDefinedBy <http://dataid.dbpedia.org/ns/core#> .



###  http://lexvo.org/ontology#Language

lvont:Language rdf:type owl:Class .



###  http://purl.org/dc/dcam/VocabularyEncodingScheme

<http://purl.org/dc/dcam/VocabularyEncodingScheme> rdf:type owl:Class .



###  http://purl.org/dc/dcmitype/Collection

<http://purl.org/dc/dcmitype/Collection> rdf:type owl:Class .



###  http://purl.org/dc/terms/Agent

dct:Agent rdf:type owl:Class ;
          
          rdfs:label "Agent"@en ;
          
          rdfs:comment "A resource that acts or has the power to act."@en ;
          
          dct:description "Examples of Agent include person, organization, and software agent."@en ;
          
          dct:hasVersion <http://dublincore.org/usage/terms/history/#Agent-001> ;
          
          rdfs:isDefinedBy dct: .



###  http://purl.org/dc/terms/AgentClass

dct:AgentClass rdf:type owl:Class ;
               
               rdfs:label "Agent Class"@en ;
               
               rdfs:subClassOf rdfs:Class ;
               
               rdfs:comment "A group of agents."@en ;
               
               dct:description "Examples of Agent Class include groups seen as classes, such as students, women, charities, lecturers."@en ;
               
               dct:hasVersion <http://dublincore.org/usage/terms/history/#AgentClass-003> ;
               
               rdfs:isDefinedBy dct: .



###  http://purl.org/dc/terms/BibliographicResource

dct:BibliographicResource rdf:type owl:Class ;
                          
                          rdfs:label "Bibliographic Resource"@en ;
                          
                          rdfs:comment "A book, article, or other documentary resource."@en ;
                          
                          dct:hasVersion <http://dublincore.org/usage/terms/history/#BibliographicResource-001> ;
                          
                          rdfs:isDefinedBy dct: .



###  http://purl.org/dc/terms/FileFormat

dct:FileFormat rdf:type owl:Class ;
               
               rdfs:label "File Format"@en ;
               
               rdfs:subClassOf dct:MediaType ;
               
               rdfs:comment "A digital resource format."@en ;
               
               dct:description "Examples include the formats defined by the list of Internet Media Types."@en ;
               
               dct:hasVersion <http://dublincore.org/usage/terms/history/#FileFormat-001> ;
               
               rdfs:isDefinedBy dct: .



###  http://purl.org/dc/terms/Frequency

dct:Frequency rdf:type owl:Class ;
              
              rdfs:label "Frequency"@en ;
              
              rdfs:comment "A rate at which something recurs."@en ;
              
              dct:hasVersion <http://dublincore.org/usage/terms/history/#Frequency-001> ;
              
              rdfs:isDefinedBy dct: .



###  http://purl.org/dc/terms/Jurisdiction

dct:Jurisdiction rdf:type owl:Class ;
                 
                 rdfs:label "Jurisdiction"@en ;
                 
                 rdfs:subClassOf dct:LocationPeriodOrJurisdiction ;
                 
                 rdfs:comment "The extent or range of judicial, law enforcement, or other authority."@en ;
                 
                 dct:hasVersion <http://dublincore.org/usage/terms/history/#Jurisdiction-001> ;
                 
                 rdfs:isDefinedBy dct: .



###  http://purl.org/dc/terms/LicenseDocument

dct:LicenseDocument rdf:type owl:Class ;
                    
                    rdfs:label "License Document"@en ;
                    
                    rdfs:subClassOf dct:RightsStatement ;
                    
                    rdfs:comment "A legal document giving official permission to do something with a Resource."@en ;
                    
                    dct:hasVersion <http://dublincore.org/usage/terms/history/#LicenseDocument-001> ;
                    
                    rdfs:isDefinedBy dct: .



###  http://purl.org/dc/terms/LinguisticSystem

dct:LinguisticSystem rdf:type owl:Class ;
                     
                     rdfs:label "Linguistic System"@en ;
                     
                     rdfs:comment "A system of signs, symbols, sounds, gestures, or rules used in communication."@en ;
                     
                     dct:description "Examples include written, spoken, sign, and computer languages."@en ;
                     
                     dct:hasVersion <http://dublincore.org/usage/terms/history/#LinguisticSystem-001> ;
                     
                     rdfs:isDefinedBy dct: .



###  http://purl.org/dc/terms/Location

dct:Location rdf:type owl:Class ;
             
             rdfs:label "Location"@en ;
             
             rdfs:subClassOf dct:LocationPeriodOrJurisdiction ;
             
             rdfs:comment "A spatial region or named place."@en ;
             
             dct:hasVersion <http://dublincore.org/usage/terms/history/#Location-001> ;
             
             rdfs:isDefinedBy dct: .



###  http://purl.org/dc/terms/LocationPeriodOrJurisdiction

dct:LocationPeriodOrJurisdiction rdf:type owl:Class ;
                                 
                                 rdfs:label "Location, Period, or Jurisdiction"@en ;
                                 
                                 rdfs:comment "A location, period of time, or jurisdiction."@en ;
                                 
                                 dct:hasVersion <http://dublincore.org/usage/terms/history/#LocationPeriodOrJurisdiction-001> ;
                                 
                                 rdfs:isDefinedBy dct: .



###  http://purl.org/dc/terms/MediaType

dct:MediaType rdf:type owl:Class ;
              
              rdfs:label "Media Type"@en ;
              
              rdfs:subClassOf dct:MediaTypeOrExtent ;
              
              rdfs:comment "A file format or physical medium."@en ;
              
              dct:hasVersion <http://dublincore.org/usage/terms/history/#MediaType-001> ;
              
              rdfs:isDefinedBy dct: .



###  http://purl.org/dc/terms/MediaTypeOrExtent

dct:MediaTypeOrExtent rdf:type owl:Class ;
                      
                      rdfs:label "Media Type or Extent"@en ;
                      
                      rdfs:comment "A media type or extent."@en ;
                      
                      dct:hasVersion <http://dublincore.org/usage/terms/history/#MediaTypeOrExtent-001> ;
                      
                      rdfs:isDefinedBy dct: .



###  http://purl.org/dc/terms/MethodOfAccrual

dct:MethodOfAccrual rdf:type owl:Class ;
                    
                    rdfs:label "Method of Accrual"@en ;
                    
                    rdfs:comment "A method by which resources are added to a collection."@en ;
                    
                    dct:hasVersion <http://dublincore.org/usage/terms/history/#MethodOfAccrual-001> ;
                    
                    rdfs:isDefinedBy dct: .



###  http://purl.org/dc/terms/MethodOfInstruction

dct:MethodOfInstruction rdf:type owl:Class ;
                        
                        rdfs:label "Method of Instruction"@en ;
                        
                        rdfs:comment "A process that is used to engender knowledge, attitudes, and skills."@en ;
                        
                        dct:hasVersion <http://dublincore.org/usage/terms/history/#MethodOfInstruction-001> ;
                        
                        rdfs:isDefinedBy dct: .



###  http://purl.org/dc/terms/PeriodOfTime

dct:PeriodOfTime rdf:type owl:Class ;
                 
                 rdfs:label "Period of Time"@en ;
                 
                 rdfs:subClassOf dct:LocationPeriodOrJurisdiction ;
                 
                 rdfs:comment "An interval of time that is named or defined by its start and end dates."@en ;
                 
                 dct:hasVersion <http://dublincore.org/usage/terms/history/#PeriodOfTime-001> ;
                 
                 rdfs:isDefinedBy dct: .



###  http://purl.org/dc/terms/PhysicalMedium

dct:PhysicalMedium rdf:type owl:Class ;
                   
                   rdfs:label "Physical Medium"@en ;
                   
                   rdfs:subClassOf dct:MediaType ;
                   
                   rdfs:comment "A physical material or carrier."@en ;
                   
                   dct:description "Examples include paper, canvas, or DVD."@en ;
                   
                   dct:hasVersion <http://dublincore.org/usage/terms/history/#PhysicalMedium-001> ;
                   
                   rdfs:isDefinedBy dct: .



###  http://purl.org/dc/terms/PhysicalResource

dct:PhysicalResource rdf:type owl:Class ;
                     
                     rdfs:label "Physical Resource"@en ;
                     
                     rdfs:comment "A material thing."@en ;
                     
                     dct:hasVersion <http://dublincore.org/usage/terms/history/#PhysicalResource-001> ;
                     
                     rdfs:isDefinedBy dct: .



###  http://purl.org/dc/terms/Policy

dct:Policy rdf:type owl:Class ;
           
           rdfs:label "Policy"@en ;
           
           rdfs:comment "A plan or course of action by an authority, intended to influence and determine decisions, actions, and other matters."@en ;
           
           dct:hasVersion <http://dublincore.org/usage/terms/history/#Policy-001> ;
           
           rdfs:isDefinedBy dct: .



###  http://purl.org/dc/terms/ProvenanceStatement

dct:ProvenanceStatement rdf:type owl:Class ;
                        
                        rdfs:label "Provenance Statement"@en ;
                        
                        rdfs:comment "A statement of any changes in ownership and custody of a resource since its creation that are significant for its authenticity, integrity, and interpretation."@en ;
                        
                        dct:hasVersion <http://dublincore.org/usage/terms/history/#ProvenanceStatement-001> ;
                        
                        rdfs:isDefinedBy dct: .



###  http://purl.org/dc/terms/RightsStatement

dct:RightsStatement rdf:type owl:Class ;
                    
                    rdfs:label "Rights Statement"@en ;
                    
                    rdfs:comment "A statement about the intellectual property rights (IPR) held in or over a Resource, a legal document giving official permission to do something with a resource, or a statement about access rights."@en ;
                    
                    dct:hasVersion <http://dublincore.org/usage/terms/history/#RightsStatement-001> ;
                    
                    rdfs:isDefinedBy dct: .



###  http://purl.org/dc/terms/SizeOrDuration

dct:SizeOrDuration rdf:type owl:Class ;
                   
                   rdfs:label "Size or Duration"@en ;
                   
                   rdfs:subClassOf dct:MediaTypeOrExtent ;
                   
                   rdfs:comment "A dimension or extent, or a time taken to play or execute."@en ;
                   
                   dct:description "Examples include a number of pages, a specification of length, width, and breadth, or a period in hours, minutes, and seconds."@en ;
                   
                   dct:hasVersion <http://dublincore.org/usage/terms/history/#SizeOrDuration-001> ;
                   
                   rdfs:isDefinedBy dct: .



###  http://purl.org/dc/terms/Standard

dct:Standard rdf:type owl:Class ;
             
             rdfs:label "Standard"@en ;
             
             rdfs:comment "A basis for comparison; a reference point against which other things can be evaluated."@en ;
             
             dct:hasVersion <http://dublincore.org/usage/terms/history/#Standard-001> ;
             
             rdfs:isDefinedBy dct: .



###  http://purl.org/spar/datacite/Identifier

datacite:Identifier rdf:type owl:Class .



###  http://rdfs.org/ns/void#Dataset

void:Dataset rdf:type owl:Class .



###  http://rdfs.org/ns/void#DatasetDescription

void:DatasetDescription rdf:type owl:Class .



###  http://spdx.org/rdf/terms/#Checksum

spdx:Checksum rdf:type owl:Class .



###  http://www.w3.org/2001/XMLSchema#datetime

xsd:datetime rdf:type owl:Class .



###  http://www.w3.org/ns/wsdl-rdf#Service

wsdl:Service rdf:type owl:Class .



###  http://xmlns.com/foaf/0.1/Agent

foaf:Agent rdf:type owl:Class .





#################################################################
#
#    Individuals
#
#################################################################


###  http://dataid.dbpedia.org/ns/core#AgentSupervision

dataid:AgentSupervision rdf:type dataid:ResponsibleAction ,
                                 owl:NamedIndividual ;
                        
                        rdfs:label "agent supervision"@en ;
                        
                        rdfs:comment "The responsibility to supervise other agents."@en ;
                        
                        rdfs:isDefinedBy <http://dataid.dbpedia.org/ns/core#> .



###  http://dataid.dbpedia.org/ns/core#Contact

dataid:Contact rdf:type dataid:AgentRole ,
                        owl:NamedIndividual ;
               
               rdfs:label "contact"@en ;
               
               rdfs:comment "Contact agent. An agent that can be contacted for general requests about the resource."@en ;
               
               rdfs:isDefinedBy <http://dataid.dbpedia.org/ns/core#> ;
               
               dataid:allowsFor dataid:ModifyContent ,
                                dataid:ReadContent ,
                                dataid:ReadDataId ,
                                dataid:ResponseToContact .



###  http://dataid.dbpedia.org/ns/core#Contributor

dataid:Contributor rdf:type dataid:AgentRole ,
                            owl:NamedIndividual ;
                   
                   rdfs:label "contributor"@en ;
                   
                   rdfs:comment "Contributor to the resource. An agent that was involved in creating or maintaining the resource but does not have the main part in this activity."@en ;
                   
                   rdfs:isDefinedBy <http://dataid.dbpedia.org/ns/core#> ;
                   
                   dataid:allowsFor dataid:ReadContent ,
                                    dataid:ReadDataId .



###  http://dataid.dbpedia.org/ns/core#Creator

dataid:Creator rdf:type dataid:AgentRole ,
                        owl:NamedIndividual ;
               
               rdfs:label "creator"@en ;
               
               rdfs:comment "Creator of the resource. An agent that is credited with a main part in the initial creation of the resource."@en ;
               
               rdfs:isDefinedBy <http://dataid.dbpedia.org/ns/core#> ;
               
               dataid:allowsFor dataid:AgentSupervision ,
                                dataid:DeleteContent ,
                                dataid:ModifyAccessLevel ,
                                dataid:ModifyAgentRoles ,
                                dataid:ModifyAuthorizedAgents ,
                                dataid:ModifyContent ,
                                dataid:PublishingDecision ,
                                dataid:ReadContent ,
                                dataid:ReadDataId ,
                                dataid:ResponseToContact ,
                                dataid:ResponseToLifeCycleEvent ,
                                dataid:UpdateDataId .



###  http://dataid.dbpedia.org/ns/core#DeleteContent

dataid:DeleteContent rdf:type dataid:EntitledAction ,
                              owl:NamedIndividual ;
                     
                     rdfs:label "delete content right"@en ;
                     
                     rdfs:comment "Entitled action to delete some content of an entity."@en ;
                     
                     rdfs:isDefinedBy <http://dataid.dbpedia.org/ns/core#> .



###  http://dataid.dbpedia.org/ns/core#Guest

dataid:Guest rdf:type dataid:AgentRole ,
                      owl:NamedIndividual ;
             
             rdfs:label "guest"@en ;
             
             rdfs:comment "A visitor/anonymous agent has only read rights on public and semi-private documents"@en ;
             
             rdfs:isDefinedBy <http://dataid.dbpedia.org/ns/core#> ;
             
             dataid:allowsFor dataid:ReadContent ,
                              dataid:ReadDataId .



###  http://dataid.dbpedia.org/ns/core#GuestAgent

dataid:GuestAgent rdf:type dataid:Agent ,
                           owl:NamedIndividual ;
                  
                  foaf:name "Guest Actor" ;
                  
                  foaf:homepage <http://dataid.dbpedia.org> ;
                  
                  rdfs:isDefinedBy <http://dataid.dbpedia.org/ns/core#> ;
                  
                  foaf:mbox <mailto:address@alibi.com> .



###  http://dataid.dbpedia.org/ns/core#Maintainer

dataid:Maintainer rdf:type dataid:AgentRole ,
                           owl:NamedIndividual ;
                  
                  rdfs:label "maintainer"@en ;
                  
                  rdfs:comment "Maintainer of the dataset. An agent that ensures the technical correctness, accessibility and up-to-dateness of a dataset."@en ;
                  
                  rdfs:isDefinedBy <http://dataid.dbpedia.org/ns/core#> ;
                  
                  dataid:allowsFor dataid:DeleteContent ,
                                   dataid:ModifyAuthorizedAgents ,
                                   dataid:ModifyContent ,
                                   dataid:ReadContent ,
                                   dataid:ReadDataId ,
                                   dataid:ResponseToContact ,
                                   dataid:ResponseToLifeCycleEvent ,
                                   dataid:UpdateDataId .



###  http://dataid.dbpedia.org/ns/core#ModifyAccessLevel

dataid:ModifyAccessLevel rdf:type dataid:EntitledAction ,
                                  owl:NamedIndividual ;
                         
                         rdfs:label "modify entity access level"@en ;
                         
                         rdfs:comment "Entitled action to modify access level of an entity."@en ;
                         
                         rdfs:isDefinedBy <http://dataid.dbpedia.org/ns/core#> .



###  http://dataid.dbpedia.org/ns/core#ModifyAgentRoles

dataid:ModifyAgentRoles rdf:type dataid:EntitledAction ,
                                 owl:NamedIndividual ;
                        
                        rdfs:label "modify agent roles"@en ;
                        
                        rdfs:comment "Entitled action to modify the role of agents on certain entities."@en ;
                        
                        rdfs:isDefinedBy <http://dataid.dbpedia.org/ns/core#> .



###  http://dataid.dbpedia.org/ns/core#ModifyAuthorizedAgents

dataid:ModifyAuthorizedAgents rdf:type dataid:EntitledAction ,
                                       owl:NamedIndividual ;
                              
                              rdfs:label "modify authorized agents"@en ;
                              
                              rdfs:comment "Entitled action to modify which agents are authorized on certain entities."@en ;
                              
                              rdfs:isDefinedBy <http://dataid.dbpedia.org/ns/core#> .



###  http://dataid.dbpedia.org/ns/core#ModifyContent

dataid:ModifyContent rdf:type dataid:EntitledAction ,
                              owl:NamedIndividual ;
                     
                     rdfs:label "modify content right"@en ;
                     
                     rdfs:comment "Entitled action to modify the content of an entity."@en ;
                     
                     rdfs:isDefinedBy <http://dataid.dbpedia.org/ns/core#> .



###  http://dataid.dbpedia.org/ns/core#PrivateAccess

dataid:PrivateAccess rdf:type dataid:AccessLevel ,
                              owl:NamedIndividual ;
                     
                     rdfs:label "private"@en ;
                     
                     rdfs:comment "Provides an agent with unrestricted access and all rights of a resource."@en ;
                     
                     rdfs:isDefinedBy <http://dataid.dbpedia.org/ns/core#> .



###  http://dataid.dbpedia.org/ns/core#PublicAccess

dataid:PublicAccess rdf:type dataid:AccessLevel ,
                             owl:NamedIndividual ;
                    
                    rdfs:label "public"@en ;
                    
                    rdfs:comment "Limits the rights an agent has on a resource to read rights."@en ;
                    
                    rdfs:isDefinedBy <http://dataid.dbpedia.org/ns/core#> .



###  http://dataid.dbpedia.org/ns/core#Publisher

dataid:Publisher rdf:type dataid:AgentRole ,
                          owl:NamedIndividual ;
                 
                 rdfs:label "publisher"@en ;
                 
                 rdfs:comment "Publisher of the dataset. An agent that makes the dataset accessible online on a server or repository without necessarily being involved in its creation."@en ;
                 
                 rdfs:isDefinedBy <http://dataid.dbpedia.org/ns/core#> ;
                 
                 dataid:allowsFor dataid:AgentSupervision ,
                                  dataid:DeleteContent ,
                                  dataid:ModifyAccessLevel ,
                                  dataid:ModifyAuthorizedAgents ,
                                  dataid:ModifyContent ,
                                  dataid:PublishingDecision ,
                                  dataid:ReadContent ,
                                  dataid:ReadDataId ,
                                  dataid:ResponseToContact ,
                                  dataid:ResponseToLifeCycleEvent ,
                                  dataid:UpdateDataId .



###  http://dataid.dbpedia.org/ns/core#PublishingDecision

dataid:PublishingDecision rdf:type dataid:ResponsibleAction ,
                                   owl:NamedIndividual ;
                          
                          rdfs:label "publishing decision"@en ;
                          
                          rdfs:comment "The responsibility decide if the entity should be published"@en ;
                          
                          rdfs:isDefinedBy <http://dataid.dbpedia.org/ns/core#> .



###  http://dataid.dbpedia.org/ns/core#ReadContent

dataid:ReadContent rdf:type dataid:EntitledAction ,
                            owl:NamedIndividual ;
                   
                   rdfs:label "read content right"@en ;
                   
                   rdfs:comment "Entitled action to read the content of an entity."@en ;
                   
                   rdfs:isDefinedBy <http://dataid.dbpedia.org/ns/core#> .



###  http://dataid.dbpedia.org/ns/core#ReadDataId

dataid:ReadDataId rdf:type dataid:EntitledAction ,
                           owl:NamedIndividual ;
                  
                  rdfs:label "read DataID right"@en ;
                  
                  rdfs:comment "Entitled action to read the DataID dataset metadata"@en ;
                  
                  rdfs:isDefinedBy <http://dataid.dbpedia.org/ns/core#> .



###  http://dataid.dbpedia.org/ns/core#ResponseToContact

dataid:ResponseToContact rdf:type dataid:ResponsibleAction ,
                                  owl:NamedIndividual ;
                         
                         rdfs:label "response to contact attempt"@en ;
                         
                         rdfs:comment "The responsibility to respond to contact attempts by external agents. A contact point for the entity."@en ;
                         
                         rdfs:isDefinedBy <http://dataid.dbpedia.org/ns/core#> .



###  http://dataid.dbpedia.org/ns/core#ResponseToLifeCycleEvent

dataid:ResponseToLifeCycleEvent rdf:type dataid:ResponsibleAction ,
                                         owl:NamedIndividual ;
                                
                                rdfs:label "response to life-cycle event"@en ;
                                
                                rdfs:comment "The responsibility to manage changes and react to bugs and issues that are reported"@en ;
                                
                                rdfs:isDefinedBy <http://dataid.dbpedia.org/ns/core#> .



###  http://dataid.dbpedia.org/ns/core#SemiPrivateAccess

dataid:SemiPrivateAccess rdf:type dataid:AccessLevel ,
                                  owl:NamedIndividual ;
                         
                         rdfs:label "semi-private"@en ;
                         
                         rdfs:comment "Limits the rights an agent has on a resource to read and modify."@en ;
                         
                         rdfs:isDefinedBy <http://dataid.dbpedia.org/ns/core#> .



###  http://dataid.dbpedia.org/ns/core#UpdateDataId

dataid:UpdateDataId rdf:type dataid:ResponsibleAction ,
                             owl:NamedIndividual ;
                    
                    rdfs:label "update DataId"@en ;
                    
                    rdfs:comment "The responsibility to update dataset metadata."@en ;
                    
                    rdfs:isDefinedBy <http://dataid.dbpedia.org/ns/core#> .



###  http://purl.org/dc/aboutdcmi#DCMI

<http://purl.org/dc/aboutdcmi#DCMI> rdf:type owl:NamedIndividual .



###  http://purl.org/dc/terms/

dct: rdf:type owl:NamedIndividual ;
     
     dct:modified "2012-06-14"^^xsd:date ;
     
     dct:title "DCMI Metadata Terms - other"@en ;
     
     dct:publisher <http://purl.org/dc/aboutdcmi#DCMI> .



###  http://purl.org/dc/terms/Agent

dct:Agent rdf:type dct:AgentClass ,
                   owl:NamedIndividual ;
          
          dct:issued "2008-01-14"^^xsd:date .



###  http://purl.org/dc/terms/AgentClass

dct:AgentClass rdf:type owl:NamedIndividual ;
               
               dct:issued "2008-01-14"^^xsd:date ;
               
               dct:modified "2012-06-14"^^xsd:date .



###  http://purl.org/dc/terms/BibliographicResource

dct:BibliographicResource rdf:type owl:NamedIndividual ;
                          
                          dct:issued "2008-01-14"^^xsd:date .



###  http://purl.org/dc/terms/Box

dct:Box rdf:type owl:NamedIndividual ;
        
        rdfs:label "DCMI Box"@en ;
        
        dct:issued "2000-07-11"^^xsd:date ;
        
        dct:modified "2008-01-14"^^xsd:date ;
        
        rdfs:comment "The set of regions in space defined by their geographic coordinates according to the DCMI Box Encoding Scheme."@en ;
        
        rdfs:seeAlso <http://dublincore.org/documents/dcmi-box/> ;
        
        dct:hasVersion <http://dublincore.org/usage/terms/history/#Box-003> ;
        
        rdfs:isDefinedBy dct: .



###  http://purl.org/dc/terms/DCMIType

dct:DCMIType rdf:type <http://purl.org/dc/dcam/VocabularyEncodingScheme> ,
                      owl:NamedIndividual ;
             
             rdfs:label "DCMI Type Vocabulary"@en ;
             
             dct:issued "2000-07-11"^^xsd:date ;
             
             dct:modified "2012-06-14"^^xsd:date ;
             
             rdfs:comment "The set of classes specified by the DCMI Type Vocabulary, used to categorize the nature or genre of the resource."@en ;
             
             dct:hasVersion <http://dublincore.org/usage/terms/history/#DCMIType-005> ;
             
             rdfs:seeAlso <http://purl.org/dc/dcmitype/> ;
             
             rdfs:isDefinedBy dct: .



###  http://purl.org/dc/terms/DDC

dct:DDC rdf:type <http://purl.org/dc/dcam/VocabularyEncodingScheme> ,
                 owl:NamedIndividual ;
        
        rdfs:label "DDC"@en ;
        
        dct:issued "2000-07-11"^^xsd:date ;
        
        dct:modified "2008-01-14"^^xsd:date ;
        
        rdfs:comment "The set of conceptual resources specified by the Dewey Decimal Classification."@en ;
        
        dct:hasVersion <http://dublincore.org/usage/terms/history/#DDC-003> ;
        
        rdfs:isDefinedBy dct: ;
        
        rdfs:seeAlso <http://www.oclc.org/dewey/> .



###  http://purl.org/dc/terms/FileFormat

dct:FileFormat rdf:type owl:NamedIndividual ;
               
               dct:issued "2008-01-14"^^xsd:date .



###  http://purl.org/dc/terms/Frequency

dct:Frequency rdf:type owl:NamedIndividual ;
              
              dct:issued "2008-01-14"^^xsd:date .



###  http://purl.org/dc/terms/IMT

dct:IMT rdf:type <http://purl.org/dc/dcam/VocabularyEncodingScheme> ,
                 owl:NamedIndividual ;
        
        rdfs:label "IMT"@en ;
        
        dct:issued "2000-07-11"^^xsd:date ;
        
        dct:modified "2008-01-14"^^xsd:date ;
        
        rdfs:comment "The set of media types specified by the Internet Assigned Numbers Authority."@en ;
        
        dct:hasVersion <http://dublincore.org/usage/terms/history/#IMT-004> ;
        
        rdfs:isDefinedBy dct: ;
        
        rdfs:seeAlso <http://www.iana.org/assignments/media-types/> .



###  http://purl.org/dc/terms/ISO3166

dct:ISO3166 rdf:type owl:NamedIndividual ;
            
            rdfs:label "ISO 3166"@en ;
            
            dct:issued "2000-07-11"^^xsd:date ;
            
            dct:modified "2008-01-14"^^xsd:date ;
            
            rdfs:comment "The set of codes listed in ISO 3166-1 for the representation of names of countries."@en ;
            
            dct:hasVersion <http://dublincore.org/usage/terms/history/#ISO3166-004> ;
            
            rdfs:isDefinedBy dct: ;
            
            rdfs:seeAlso <http://www.iso.org/iso/en/prods-services/iso3166ma/02iso-3166-code-lists/list-en1.html> .



###  http://purl.org/dc/terms/ISO639-2

dct:ISO639-2 rdf:type owl:NamedIndividual ;
             
             rdfs:label "ISO 639-2"@en ;
             
             dct:issued "2000-07-11"^^xsd:date ;
             
             dct:modified "2008-01-14"^^xsd:date ;
             
             rdfs:comment "The three-letter alphabetic codes listed in ISO639-2 for the representation of names of languages."@en ;
             
             dct:hasVersion <http://dublincore.org/usage/terms/history/#ISO639-2-003> ;
             
             rdfs:seeAlso <http://lcweb.loc.gov/standards/iso639-2/langhome.html> ;
             
             rdfs:isDefinedBy dct: .



###  http://purl.org/dc/terms/ISO639-3

dct:ISO639-3 rdf:type owl:NamedIndividual ;
             
             rdfs:label "ISO 639-3"@en ;
             
             dct:issued "2008-01-14"^^xsd:date ;
             
             rdfs:comment "The set of three-letter codes listed in ISO 639-3 for the representation of names of languages."@en ;
             
             dct:hasVersion <http://dublincore.org/usage/terms/history/#ISO639-3-001> ;
             
             rdfs:isDefinedBy dct: ;
             
             rdfs:seeAlso <http://www.sil.org/iso639-3/> .



###  http://purl.org/dc/terms/Jurisdiction

dct:Jurisdiction rdf:type owl:NamedIndividual ;
                 
                 dct:issued "2008-01-14"^^xsd:date .



###  http://purl.org/dc/terms/LCC

dct:LCC rdf:type <http://purl.org/dc/dcam/VocabularyEncodingScheme> ,
                 owl:NamedIndividual ;
        
        rdfs:label "LCC"@en ;
        
        dct:issued "2000-07-11"^^xsd:date ;
        
        dct:modified "2008-01-14"^^xsd:date ;
        
        rdfs:comment "The set of conceptual resources specified by the Library of Congress Classification."@en ;
        
        dct:hasVersion <http://dublincore.org/usage/terms/history/#LCC-003> ;
        
        rdfs:seeAlso <http://lcweb.loc.gov/catdir/cpso/lcco/lcco.html> ;
        
        rdfs:isDefinedBy dct: .



###  http://purl.org/dc/terms/LCSH

dct:LCSH rdf:type <http://purl.org/dc/dcam/VocabularyEncodingScheme> ,
                  owl:NamedIndividual ;
         
         rdfs:label "LCSH"@en ;
         
         dct:issued "2000-07-11"^^xsd:date ;
         
         dct:modified "2008-01-14"^^xsd:date ;
         
         rdfs:comment "The set of labeled concepts specified by the Library of Congress Subject Headings."@en ;
         
         dct:hasVersion <http://dublincore.org/usage/terms/history/#LCSH-003> ;
         
         rdfs:isDefinedBy dct: .



###  http://purl.org/dc/terms/LicenseDocument

dct:LicenseDocument rdf:type owl:NamedIndividual ;
                    
                    dct:issued "2008-01-14"^^xsd:date .



###  http://purl.org/dc/terms/LinguisticSystem

dct:LinguisticSystem rdf:type owl:NamedIndividual ;
                     
                     dct:issued "2008-01-14"^^xsd:date .



###  http://purl.org/dc/terms/Location

dct:Location rdf:type owl:NamedIndividual ;
             
             dct:issued "2008-01-14"^^xsd:date .



###  http://purl.org/dc/terms/LocationPeriodOrJurisdiction

dct:LocationPeriodOrJurisdiction rdf:type owl:NamedIndividual ;
                                 
                                 dct:issued "2008-01-14"^^xsd:date .



###  http://purl.org/dc/terms/MESH

dct:MESH rdf:type <http://purl.org/dc/dcam/VocabularyEncodingScheme> ,
                  owl:NamedIndividual ;
         
         rdfs:label "MeSH"@en ;
         
         dct:issued "2000-07-11"^^xsd:date ;
         
         dct:modified "2008-01-14"^^xsd:date ;
         
         rdfs:comment "The set of labeled concepts specified by the Medical Subject Headings."@en ;
         
         dct:hasVersion <http://dublincore.org/usage/terms/history/#MESH-003> ;
         
         rdfs:isDefinedBy dct: ;
         
         rdfs:seeAlso <http://www.nlm.nih.gov/mesh/meshhome.html> .



###  http://purl.org/dc/terms/MediaType

dct:MediaType rdf:type owl:NamedIndividual ;
              
              dct:issued "2008-01-14"^^xsd:date .



###  http://purl.org/dc/terms/MediaTypeOrExtent

dct:MediaTypeOrExtent rdf:type owl:NamedIndividual ;
                      
                      dct:issued "2008-01-14"^^xsd:date .



###  http://purl.org/dc/terms/MethodOfAccrual

dct:MethodOfAccrual rdf:type owl:NamedIndividual ;
                    
                    dct:issued "2008-01-14"^^xsd:date .



###  http://purl.org/dc/terms/MethodOfInstruction

dct:MethodOfInstruction rdf:type owl:NamedIndividual ;
                        
                        dct:issued "2008-01-14"^^xsd:date .



###  http://purl.org/dc/terms/NLM

dct:NLM rdf:type <http://purl.org/dc/dcam/VocabularyEncodingScheme> ,
                 owl:NamedIndividual ;
        
        rdfs:label "NLM"@en ;
        
        dct:issued "2005-06-13"^^xsd:date ;
        
        dct:modified "2008-01-14"^^xsd:date ;
        
        rdfs:comment "The set of conceptual resources specified by the National Library of Medicine Classification."@en ;
        
        dct:hasVersion <http://dublincore.org/usage/terms/history/#NLM-002> ;
        
        rdfs:isDefinedBy dct: ;
        
        rdfs:seeAlso <http://wwwcf.nlm.nih.gov/class/> .



###  http://purl.org/dc/terms/Period

dct:Period rdf:type owl:NamedIndividual ;
           
           rdfs:label "DCMI Period"@en ;
           
           dct:issued "2000-07-11"^^xsd:date ;
           
           dct:modified "2008-01-14"^^xsd:date ;
           
           rdfs:comment "The set of time intervals defined by their limits according to the DCMI Period Encoding Scheme."@en ;
           
           rdfs:seeAlso <http://dublincore.org/documents/dcmi-period/> ;
           
           dct:hasVersion <http://dublincore.org/usage/terms/history/#Period-003> ;
           
           rdfs:isDefinedBy dct: .



###  http://purl.org/dc/terms/PeriodOfTime

dct:PeriodOfTime rdf:type owl:NamedIndividual ;
                 
                 dct:issued "2008-01-14"^^xsd:date .



###  http://purl.org/dc/terms/PhysicalMedium

dct:PhysicalMedium rdf:type owl:NamedIndividual ;
                   
                   dct:issued "2008-01-14"^^xsd:date .



###  http://purl.org/dc/terms/PhysicalResource

dct:PhysicalResource rdf:type owl:NamedIndividual ;
                     
                     dct:issued "2008-01-14"^^xsd:date .



###  http://purl.org/dc/terms/Point

dct:Point rdf:type owl:NamedIndividual ;
          
          rdfs:label "DCMI Point"@en ;
          
          dct:issued "2000-07-11"^^xsd:date ;
          
          dct:modified "2008-01-14"^^xsd:date ;
          
          rdfs:comment "The set of points in space defined by their geographic coordinates according to the DCMI Point Encoding Scheme."@en ;
          
          rdfs:seeAlso <http://dublincore.org/documents/dcmi-point/> ;
          
          dct:hasVersion <http://dublincore.org/usage/terms/history/#Point-003> ;
          
          rdfs:isDefinedBy dct: .



###  http://purl.org/dc/terms/Policy

dct:Policy rdf:type owl:NamedIndividual ;
           
           dct:issued "2008-01-14"^^xsd:date .



###  http://purl.org/dc/terms/ProvenanceStatement

dct:ProvenanceStatement rdf:type owl:NamedIndividual ;
                        
                        dct:issued "2008-01-14"^^xsd:date .



###  http://purl.org/dc/terms/RFC1766

dct:RFC1766 rdf:type owl:NamedIndividual ;
            
            rdfs:label "RFC 1766"@en ;
            
            dct:issued "2000-07-11"^^xsd:date ;
            
            dct:modified "2008-01-14"^^xsd:date ;
            
            rdfs:comment "The set of tags, constructed according to RFC 1766, for the identification of languages."@en ;
            
            dct:hasVersion <http://dublincore.org/usage/terms/history/#RFC1766-003> ;
            
            rdfs:isDefinedBy dct: ;
            
            rdfs:seeAlso <http://www.ietf.org/rfc/rfc1766.txt> .



###  http://purl.org/dc/terms/RFC3066

dct:RFC3066 rdf:type owl:NamedIndividual ;
            
            rdfs:label "RFC 3066"@en ;
            
            dct:issued "2002-07-13"^^xsd:date ;
            
            dct:modified "2008-01-14"^^xsd:date ;
            
            dct:description "RFC 3066 has been obsoleted by RFC 4646."@en ;
            
            rdfs:comment "The set of tags constructed according to RFC 3066 for the identification of languages."@en ;
            
            dct:hasVersion <http://dublincore.org/usage/terms/history/#RFC3066-002> ;
            
            rdfs:isDefinedBy dct: ;
            
            rdfs:seeAlso <http://www.ietf.org/rfc/rfc3066.txt> .



###  http://purl.org/dc/terms/RFC4646

dct:RFC4646 rdf:type owl:NamedIndividual ;
            
            rdfs:label "RFC 4646"@en ;
            
            dct:issued "2008-01-14"^^xsd:date ;
            
            dct:description "RFC 4646 obsoletes RFC 3066."@en ;
            
            rdfs:comment "The set of tags constructed according to RFC 4646 for the identification of languages."@en ;
            
            dct:hasVersion <http://dublincore.org/usage/terms/history/#RFC4646-001> ;
            
            rdfs:isDefinedBy dct: ;
            
            rdfs:seeAlso <http://www.ietf.org/rfc/rfc4646.txt> .



###  http://purl.org/dc/terms/RFC5646

dct:RFC5646 rdf:type owl:NamedIndividual ;
            
            rdfs:label "RFC 5646"@en ;
            
            dct:issued "2010-10-11"^^xsd:date ;
            
            dct:description "RFC 5646 obsoletes RFC 4646."@en ;
            
            rdfs:comment "The set of tags constructed according to RFC 5646 for the identification of languages."@en ;
            
            dct:hasVersion <http://dublincore.org/usage/terms/history/#RFC5646-001> ;
            
            rdfs:isDefinedBy dct: ;
            
            rdfs:seeAlso <http://www.ietf.org/rfc/rfc5646.txt> .



###  http://purl.org/dc/terms/RightsStatement

dct:RightsStatement rdf:type owl:NamedIndividual ;
                    
                    dct:issued "2008-01-14"^^xsd:date .



###  http://purl.org/dc/terms/SizeOrDuration

dct:SizeOrDuration rdf:type owl:NamedIndividual ;
                   
                   dct:issued "2008-01-14"^^xsd:date .



###  http://purl.org/dc/terms/Standard

dct:Standard rdf:type owl:NamedIndividual ;
             
             dct:issued "2008-01-14"^^xsd:date .



###  http://purl.org/dc/terms/TGN

dct:TGN rdf:type <http://purl.org/dc/dcam/VocabularyEncodingScheme> ,
                 owl:NamedIndividual ;
        
        rdfs:label "TGN"@en ;
        
        dct:issued "2000-07-11"^^xsd:date ;
        
        dct:modified "2008-01-14"^^xsd:date ;
        
        rdfs:comment "The set of places specified by the Getty Thesaurus of Geographic Names."@en ;
        
        dct:hasVersion <http://dublincore.org/usage/terms/history/#TGN-003> ;
        
        rdfs:isDefinedBy dct: ;
        
        rdfs:seeAlso <http://www.getty.edu/research/tools/vocabulary/tgn/index.html> .



###  http://purl.org/dc/terms/UDC

dct:UDC rdf:type <http://purl.org/dc/dcam/VocabularyEncodingScheme> ,
                 owl:NamedIndividual ;
        
        rdfs:label "UDC"@en ;
        
        dct:issued "2000-07-11"^^xsd:date ;
        
        dct:modified "2008-01-14"^^xsd:date ;
        
        rdfs:comment "The set of conceptual resources specified by the Universal Decimal Classification."@en ;
        
        dct:hasVersion <http://dublincore.org/usage/terms/history/#UDC-003> ;
        
        rdfs:isDefinedBy dct: ;
        
        rdfs:seeAlso <http://www.udcc.org/> .



###  http://purl.org/dc/terms/URI

dct:URI rdf:type owl:NamedIndividual ;
        
        rdfs:label "URI"@en ;
        
        dct:issued "2000-07-11"^^xsd:date ;
        
        dct:modified "2008-01-14"^^xsd:date ;
        
        rdfs:comment "The set of identifiers constructed according to the generic syntax for Uniform Resource Identifiers as specified by the Internet Engineering Task Force."@en ;
        
        dct:hasVersion <http://dublincore.org/usage/terms/history/#URI-003> ;
        
        rdfs:isDefinedBy dct: ;
        
        rdfs:seeAlso <http://www.ietf.org/rfc/rfc3986.txt> .



###  http://purl.org/dc/terms/W3CDTF

dct:W3CDTF rdf:type owl:NamedIndividual ;
           
           rdfs:label "W3C-DTF"@en ;
           
           dct:issued "2000-07-11"^^xsd:date ;
           
           dct:modified "2008-01-14"^^xsd:date ;
           
           rdfs:comment "The set of dates and times constructed according to the W3C Date and Time Formats Specification."@en ;
           
           dct:hasVersion <http://dublincore.org/usage/terms/history/#W3CDTF-003> ;
           
           rdfs:isDefinedBy dct: ;
           
           rdfs:seeAlso <http://www.w3.org/TR/NOTE-datetime> .



###  http://purl.org/dc/terms/abstract

dct:abstract rdf:type owl:NamedIndividual ;
             
             rdfs:label "Abstract"@en ;
             
             dct:issued "2000-07-11"^^xsd:date ;
             
             dct:modified "2008-01-14"^^xsd:date ;
             
             rdfs:comment "A summary of the resource."@en ;
             
             dct:hasVersion <http://dublincore.org/usage/terms/history/#abstract-003> ;
             
             rdfs:isDefinedBy dct: .



###  http://purl.org/dc/terms/accessRights

dct:accessRights rdf:type owl:NamedIndividual ;
                 
                 rdfs:label "Access Rights"@en ;
                 
                 dct:issued "2003-02-15"^^xsd:date ;
                 
                 dct:modified "2008-01-14"^^xsd:date ;
                 
                 dct:description "Access Rights may include information regarding access or restrictions based on privacy, security, or other policies."@en ;
                 
                 rdfs:comment "Information about who can access the resource or an indication of its security status."@en ;
                 
                 dct:hasVersion <http://dublincore.org/usage/terms/history/#accessRights-002> ;
                 
                 rdfs:isDefinedBy dct: .



###  http://purl.org/dc/terms/accrualMethod

dct:accrualMethod rdf:type owl:NamedIndividual ;
                  
                  rdfs:label "Accrual Method"@en ;
                  
                  dct:issued "2005-06-13"^^xsd:date ;
                  
                  dct:modified "2010-10-11"^^xsd:date ;
                  
                  rdfs:comment "The method by which items are added to a collection."@en ;
                  
                  dct:hasVersion <http://dublincore.org/usage/terms/history/#accrualMethod-003> ;
                  
                  rdfs:isDefinedBy dct: .



###  http://purl.org/dc/terms/accrualPeriodicity

dct:accrualPeriodicity rdf:type owl:NamedIndividual ;
                       
                       rdfs:label "Accrual Periodicity"@en ;
                       
                       dct:issued "2005-06-13"^^xsd:date ;
                       
                       dct:modified "2010-10-11"^^xsd:date ;
                       
                       rdfs:comment "The frequency with which items are added to a collection."@en ;
                       
                       dct:hasVersion <http://dublincore.org/usage/terms/history/#accrualPeriodicity-003> ;
                       
                       rdfs:isDefinedBy dct: .



###  http://purl.org/dc/terms/accrualPolicy

dct:accrualPolicy rdf:type owl:NamedIndividual ;
                  
                  rdfs:label "Accrual Policy"@en ;
                  
                  dct:issued "2005-06-13"^^xsd:date ;
                  
                  dct:modified "2010-10-11"^^xsd:date ;
                  
                  rdfs:comment "The policy governing the addition of items to a collection."@en ;
                  
                  dct:hasVersion <http://dublincore.org/usage/terms/history/#accrualPolicy-003> ;
                  
                  rdfs:isDefinedBy dct: .



###  http://purl.org/dc/terms/alternative

dct:alternative rdf:type owl:NamedIndividual ;
                
                rdfs:label "Alternative Title"@en ;
                
                dct:issued "2000-07-11"^^xsd:date ;
                
                dct:modified "2010-10-11"^^xsd:date ;
                
                rdfs:comment "An alternative name for the resource."@en ;
                
                dct:description "The distinction between titles and alternative titles is application-specific."@en ;
                
                dct:hasVersion <http://dublincore.org/usage/terms/history/#alternative-003> ;
                
                rdfs:isDefinedBy dct: .



###  http://purl.org/dc/terms/audience

dct:audience rdf:type owl:NamedIndividual ;
             
             rdfs:label "Audience"@en ;
             
             dct:issued "2001-05-21"^^xsd:date ;
             
             dct:modified "2008-01-14"^^xsd:date ;
             
             rdfs:comment "A class of entity for whom the resource is intended or useful."@en ;
             
             dct:hasVersion <http://dublincore.org/usage/terms/history/#audience-003> ;
             
             rdfs:isDefinedBy dct: .



###  http://purl.org/dc/terms/available

dct:available rdf:type owl:NamedIndividual ;
              
              rdfs:label "Date Available"@en ;
              
              dct:issued "2000-07-11"^^xsd:date ;
              
              dct:modified "2008-01-14"^^xsd:date ;
              
              rdfs:comment "Date (often a range) that the resource became or will become available."@en ;
              
              dct:hasVersion <http://dublincore.org/usage/terms/history/#available-003> ;
              
              rdfs:isDefinedBy dct: .



###  http://purl.org/dc/terms/bibliographicCitation

dct:bibliographicCitation rdf:type owl:NamedIndividual ;
                          
                          rdfs:label "Bibliographic Citation"@en ;
                          
                          dct:issued "2003-02-15"^^xsd:date ;
                          
                          dct:modified "2008-01-14"^^xsd:date ;
                          
                          rdfs:comment "A bibliographic reference for the resource."@en ;
                          
                          dct:description "Recommended practice is to include sufficient bibliographic detail to identify the resource as unambiguously as possible."@en ;
                          
                          dct:hasVersion <http://dublincore.org/usage/terms/history/#bibliographicCitation-002> ;
                          
                          rdfs:isDefinedBy dct: .



###  http://purl.org/dc/terms/conformsTo

dct:conformsTo rdf:type owl:NamedIndividual ;
               
               rdfs:label "Conforms To"@en ;
               
               dct:issued "2001-05-21"^^xsd:date ;
               
               dct:modified "2008-01-14"^^xsd:date ;
               
               rdfs:comment "An established standard to which the described resource conforms."@en ;
               
               dct:hasVersion <http://dublincore.org/usage/terms/history/#conformsTo-003> ;
               
               rdfs:isDefinedBy dct: .



###  http://purl.org/dc/terms/contributor

dct:contributor rdf:type owl:NamedIndividual ;
                
                rdfs:label "Contributor"@en ;
                
                dct:issued "2008-01-14"^^xsd:date ;
                
                dct:modified "2010-10-11"^^xsd:date ;
                
                rdfs:comment "An entity responsible for making contributions to the resource."@en ;
                
                dct:description "Examples of a Contributor include a person, an organization, or a service."@en ;
                
                dct:hasVersion <http://dublincore.org/usage/terms/history/#contributorT-001> ;
                
                rdfs:isDefinedBy dct: .



###  http://purl.org/dc/terms/coverage

dct:coverage rdf:type owl:NamedIndividual ;
             
             rdfs:label "Coverage"@en ;
             
             dct:modified "2008-01-14"^^xsd:date ;
             
             dct:issued "2008-01-14"^^xsd:date ;
             
             dct:description "Spatial topic and spatial applicability may be a named place or a location specified by its geographic coordinates. Temporal topic may be a named period, date, or date range. A jurisdiction may be a named administrative entity or a geographic place to which the resource applies. Recommended best practice is to use a controlled vocabulary such as the Thesaurus of Geographic Names [TGN]. Where appropriate, named places or time periods can be used in preference to numeric identifiers such as sets of coordinates or date ranges."@en ;
             
             rdfs:comment "The spatial or temporal topic of the resource, the spatial applicability of the resource, or the jurisdiction under which the resource is relevant."@en ;
             
             dct:hasVersion <http://dublincore.org/usage/terms/history/#coverageT-001> ;
             
             rdfs:isDefinedBy dct: .



###  http://purl.org/dc/terms/created

dct:created rdf:type owl:NamedIndividual ;
            
            rdfs:label "Date Created"@en ;
            
            dct:issued "2000-07-11"^^xsd:date ;
            
            dct:modified "2008-01-14"^^xsd:date ;
            
            rdfs:comment "Date of creation of the resource."@en ;
            
            dct:hasVersion <http://dublincore.org/usage/terms/history/#created-003> ;
            
            rdfs:isDefinedBy dct: .



###  http://purl.org/dc/terms/creator

dct:creator rdf:type owl:NamedIndividual ;
            
            rdfs:label "Creator"@en ;
            
            dct:issued "2008-01-14"^^xsd:date ;
            
            dct:modified "2010-10-11"^^xsd:date ;
            
            rdfs:comment "An entity primarily responsible for making the resource."@en ;
            
            dct:description "Examples of a Creator include a person, an organization, or a service."@en ;
            
            dct:hasVersion <http://dublincore.org/usage/terms/history/#creatorT-002> ;
            
            rdfs:isDefinedBy dct: .



###  http://purl.org/dc/terms/date

dct:date rdf:type owl:NamedIndividual ;
         
         rdfs:label "Date"@en ;
         
         dct:issued "2008-01-14"^^xsd:date ;
         
         dct:modified "2008-01-14"^^xsd:date ;
         
         rdfs:comment "A point or period of time associated with an event in the lifecycle of the resource."@en ;
         
         dct:description "Date may be used to express temporal information at any level of granularity.  Recommended best practice is to use an encoding scheme, such as the W3CDTF profile of ISO 8601 [W3CDTF]."@en ;
         
         dct:hasVersion <http://dublincore.org/usage/terms/history/#dateT-001> ;
         
         rdfs:isDefinedBy dct: .



###  http://purl.org/dc/terms/dateAccepted

dct:dateAccepted rdf:type owl:NamedIndividual ;
                 
                 rdfs:label "Date Accepted"@en ;
                 
                 dct:issued "2002-07-13"^^xsd:date ;
                 
                 dct:modified "2008-01-14"^^xsd:date ;
                 
                 rdfs:comment "Date of acceptance of the resource."@en ;
                 
                 dct:description "Examples of resources to which a Date Accepted may be relevant are a thesis (accepted by a university department) or an article (accepted by a journal)."@en ;
                 
                 dct:hasVersion <http://dublincore.org/usage/terms/history/#dateAccepted-002> ;
                 
                 rdfs:isDefinedBy dct: .



###  http://purl.org/dc/terms/dateCopyrighted

dct:dateCopyrighted rdf:type owl:NamedIndividual ;
                    
                    rdfs:label "Date Copyrighted"@en ;
                    
                    dct:issued "2002-07-13"^^xsd:date ;
                    
                    dct:modified "2008-01-14"^^xsd:date ;
                    
                    rdfs:comment "Date of copyright."@en ;
                    
                    dct:hasVersion <http://dublincore.org/usage/terms/history/#dateCopyrighted-002> ;
                    
                    rdfs:isDefinedBy dct: .



###  http://purl.org/dc/terms/dateSubmitted

dct:dateSubmitted rdf:type owl:NamedIndividual ;
                  
                  rdfs:label "Date Submitted"@en ;
                  
                  dct:issued "2002-07-13"^^xsd:date ;
                  
                  dct:modified "2008-01-14"^^xsd:date ;
                  
                  rdfs:comment "Date of submission of the resource."@en ;
                  
                  dct:description "Examples of resources to which a Date Submitted may be relevant are a thesis (submitted to a university department) or an article (submitted to a journal)."@en ;
                  
                  dct:hasVersion <http://dublincore.org/usage/terms/history/#dateSubmitted-002> ;
                  
                  rdfs:isDefinedBy dct: .



###  http://purl.org/dc/terms/description

dct:description rdf:type owl:AnnotationProperty ,
                         owl:NamedIndividual ;
                
                rdfs:label "Description"@en ;
                
                dct:issued "2008-01-14"^^xsd:date ;
                
                dct:modified "2008-01-14"^^xsd:date ;
                
                rdfs:comment "An account of the resource."@en ;
                
                dct:description "Description may include but is not limited to: an abstract, a table of contents, a graphical representation, or a free-text account of the resource."@en ;
                
                dct:hasVersion <http://dublincore.org/usage/terms/history/#descriptionT-001> ;
                
                rdfs:isDefinedBy dct: .



###  http://purl.org/dc/terms/educationLevel

dct:educationLevel rdf:type owl:NamedIndividual ;
                   
                   rdfs:label "Audience Education Level"@en ;
                   
                   dct:issued "2002-07-13"^^xsd:date ;
                   
                   dct:modified "2008-01-14"^^xsd:date ;
                   
                   rdfs:comment "A class of entity, defined in terms of progression through an educational or training context, for which the described resource is intended."@en ;
                   
                   dct:hasVersion <http://dublincore.org/usage/terms/history/#educationLevel-002> ;
                   
                   rdfs:isDefinedBy dct: .



###  http://purl.org/dc/terms/extent

dct:extent rdf:type owl:NamedIndividual ;
           
           rdfs:label "Extent"@en ;
           
           dct:issued "2000-07-11"^^xsd:date ;
           
           dct:modified "2008-01-14"^^xsd:date ;
           
           rdfs:comment "The size or duration of the resource."@en ;
           
           dct:hasVersion <http://dublincore.org/usage/terms/history/#extent-003> ;
           
           rdfs:isDefinedBy dct: .



###  http://purl.org/dc/terms/format

dct:format rdf:type owl:NamedIndividual ;
           
           rdfs:label "Format"@en ;
           
           dct:issued "2008-01-14"^^xsd:date ;
           
           dct:modified "2008-01-14"^^xsd:date ;
           
           dct:description "Examples of dimensions include size and duration. Recommended best practice is to use a controlled vocabulary such as the list of Internet Media Types [MIME]."@en ;
           
           rdfs:comment "The file format, physical medium, or dimensions of the resource."@en ;
           
           dct:hasVersion <http://dublincore.org/usage/terms/history/#formatT-001> ;
           
           rdfs:isDefinedBy dct: .



###  http://purl.org/dc/terms/hasFormat

dct:hasFormat rdf:type owl:NamedIndividual ;
              
              rdfs:label "Has Format"@en ;
              
              dct:issued "2000-07-11"^^xsd:date ;
              
              dct:modified "2008-01-14"^^xsd:date ;
              
              rdfs:comment "A related resource that is substantially the same as the pre-existing described resource, but in another format."@en ;
              
              skos:note "This term is intended to be used with non-literal values as defined in the DCMI Abstract Model (http://dublincore.org/documents/abstract-model/).  As of December 2007, the DCMI Usage Board is seeking a way to express this intention with a formal range declaration."@en ;
              
              dct:hasVersion <http://dublincore.org/usage/terms/history/#hasFormat-003> ;
              
              rdfs:isDefinedBy dct: .



###  http://purl.org/dc/terms/hasPart

dct:hasPart rdf:type owl:NamedIndividual ;
            
            rdfs:label "Has Part"@en ;
            
            dct:issued "2000-07-11"^^xsd:date ;
            
            dct:modified "2008-01-14"^^xsd:date ;
            
            rdfs:comment "A related resource that is included either physically or logically in the described resource."@en ;
            
            skos:note "This term is intended to be used with non-literal values as defined in the DCMI Abstract Model (http://dublincore.org/documents/abstract-model/).  As of December 2007, the DCMI Usage Board is seeking a way to express this intention with a formal range declaration."@en ;
            
            dct:hasVersion <http://dublincore.org/usage/terms/history/#hasPart-003> ;
            
            rdfs:isDefinedBy dct: .



###  http://purl.org/dc/terms/hasVersion

dct:hasVersion rdf:type owl:AnnotationProperty ,
                        owl:NamedIndividual ;
               
               rdfs:label "Has Version"@en ;
               
               dct:issued "2000-07-11"^^xsd:date ;
               
               dct:modified "2008-01-14"^^xsd:date ;
               
               rdfs:comment "A related resource that is a version, edition, or adaptation of the described resource."@en ;
               
               skos:note "This term is intended to be used with non-literal values as defined in the DCMI Abstract Model (http://dublincore.org/documents/abstract-model/).  As of December 2007, the DCMI Usage Board is seeking a way to express this intention with a formal range declaration."@en ;
               
               dct:hasVersion <http://dublincore.org/usage/terms/history/#hasVersion-003> ;
               
               rdfs:isDefinedBy dct: .



###  http://purl.org/dc/terms/identifier

dct:identifier rdf:type owl:NamedIndividual ;
               
               rdfs:label "Identifier"@en ;
               
               dct:issued "2008-01-14"^^xsd:date ;
               
               dct:modified "2008-01-14"^^xsd:date ;
               
               rdfs:comment "An unambiguous reference to the resource within a given context."@en ;
               
               dct:description "Recommended best practice is to identify the resource by means of a string conforming to a formal identification system. "@en ;
               
               dct:hasVersion <http://dublincore.org/usage/terms/history/#identifierT-001> ;
               
               rdfs:isDefinedBy dct: .



###  http://purl.org/dc/terms/instructionalMethod

dct:instructionalMethod rdf:type owl:NamedIndividual ;
                        
                        rdfs:label "Instructional Method"@en ;
                        
                        dct:issued "2005-06-13"^^xsd:date ;
                        
                        dct:modified "2008-01-14"^^xsd:date ;
                        
                        rdfs:comment "A process, used to engender knowledge, attitudes and skills, that the described resource is designed to support."@en ;
                        
                        dct:description "Instructional Method will typically include ways of presenting instructional materials or conducting instructional activities, patterns of learner-to-learner and learner-to-instructor interactions, and mechanisms by which group and individual levels of learning are measured.  Instructional methods include all aspects of the instruction and learning processes from planning and implementation through evaluation and feedback."@en ;
                        
                        dct:hasVersion <http://dublincore.org/usage/terms/history/#instructionalMethod-002> ;
                        
                        rdfs:isDefinedBy dct: .



###  http://purl.org/dc/terms/isFormatOf

dct:isFormatOf rdf:type owl:NamedIndividual ;
               
               rdfs:label "Is Format Of"@en ;
               
               dct:issued "2000-07-11"^^xsd:date ;
               
               dct:modified "2008-01-14"^^xsd:date ;
               
               rdfs:comment "A related resource that is substantially the same as the described resource, but in another format."@en ;
               
               skos:note "This term is intended to be used with non-literal values as defined in the DCMI Abstract Model (http://dublincore.org/documents/abstract-model/).  As of December 2007, the DCMI Usage Board is seeking a way to express this intention with a formal range declaration."@en ;
               
               dct:hasVersion <http://dublincore.org/usage/terms/history/#isFormatOf-003> ;
               
               rdfs:isDefinedBy dct: .



###  http://purl.org/dc/terms/isPartOf

dct:isPartOf rdf:type owl:NamedIndividual ;
             
             rdfs:label "Is Part Of"@en ;
             
             dct:issued "2000-07-11"^^xsd:date ;
             
             dct:modified "2008-01-14"^^xsd:date ;
             
             rdfs:comment "A related resource in which the described resource is physically or logically included."@en ;
             
             skos:note "This term is intended to be used with non-literal values as defined in the DCMI Abstract Model (http://dublincore.org/documents/abstract-model/).  As of December 2007, the DCMI Usage Board is seeking a way to express this intention with a formal range declaration."@en ;
             
             dct:hasVersion <http://dublincore.org/usage/terms/history/#isPartOf-003> ;
             
             rdfs:isDefinedBy dct: .



###  http://purl.org/dc/terms/isReferencedBy

dct:isReferencedBy rdf:type owl:NamedIndividual ;
                   
                   rdfs:label "Is Referenced By"@en ;
                   
                   dct:issued "2000-07-11"^^xsd:date ;
                   
                   dct:modified "2008-01-14"^^xsd:date ;
                   
                   rdfs:comment "A related resource that references, cites, or otherwise points to the described resource."@en ;
                   
                   skos:note "This term is intended to be used with non-literal values as defined in the DCMI Abstract Model (http://dublincore.org/documents/abstract-model/).  As of December 2007, the DCMI Usage Board is seeking a way to express this intention with a formal range declaration."@en ;
                   
                   dct:hasVersion <http://dublincore.org/usage/terms/history/#isReferencedBy-003> ;
                   
                   rdfs:isDefinedBy dct: .



###  http://purl.org/dc/terms/isReplacedBy

dct:isReplacedBy rdf:type owl:NamedIndividual ;
                 
                 rdfs:label "Is Replaced By"@en ;
                 
                 dct:issued "2000-07-11"^^xsd:date ;
                 
                 dct:modified "2008-01-14"^^xsd:date ;
                 
                 rdfs:comment "A related resource that supplants, displaces, or supersedes the described resource."@en ;
                 
                 skos:note "This term is intended to be used with non-literal values as defined in the DCMI Abstract Model (http://dublincore.org/documents/abstract-model/).  As of December 2007, the DCMI Usage Board is seeking a way to express this intention with a formal range declaration."@en ;
                 
                 dct:hasVersion <http://dublincore.org/usage/terms/history/#isReplacedBy-003> ;
                 
                 rdfs:isDefinedBy dct: .



###  http://purl.org/dc/terms/isRequiredBy

dct:isRequiredBy rdf:type owl:NamedIndividual ;
                 
                 rdfs:label "Is Required By"@en ;
                 
                 dct:issued "2000-07-11"^^xsd:date ;
                 
                 dct:modified "2008-01-14"^^xsd:date ;
                 
                 rdfs:comment "A related resource that requires the described resource to support its function, delivery, or coherence."@en ;
                 
                 skos:note "This term is intended to be used with non-literal values as defined in the DCMI Abstract Model (http://dublincore.org/documents/abstract-model/).  As of December 2007, the DCMI Usage Board is seeking a way to express this intention with a formal range declaration."@en ;
                 
                 dct:hasVersion <http://dublincore.org/usage/terms/history/#isRequiredBy-003> ;
                 
                 rdfs:isDefinedBy dct: .



###  http://purl.org/dc/terms/isVersionOf

dct:isVersionOf rdf:type owl:NamedIndividual ;
                
                rdfs:label "Is Version Of"@en ;
                
                dct:issued "2000-07-11"^^xsd:date ;
                
                dct:modified "2008-01-14"^^xsd:date ;
                
                rdfs:comment "A related resource of which the described resource is a version, edition, or adaptation."@en ;
                
                dct:description "Changes in version imply substantive changes in content rather than differences in format."@en ;
                
                skos:note "This term is intended to be used with non-literal values as defined in the DCMI Abstract Model (http://dublincore.org/documents/abstract-model/).  As of December 2007, the DCMI Usage Board is seeking a way to express this intention with a formal range declaration."@en ;
                
                dct:hasVersion <http://dublincore.org/usage/terms/history/#isVersionOf-003> ;
                
                rdfs:isDefinedBy dct: .



###  http://purl.org/dc/terms/issued

dct:issued rdf:type owl:DatatypeProperty ,
                    owl:NamedIndividual ;
           
           rdfs:label "Date Issued"@en ;
           
           dct:issued "2000-07-11"^^xsd:date ;
           
           dct:modified "2008-01-14"^^xsd:date ;
           
           rdfs:comment "Date of formal issuance (e.g., publication) of the resource."@en ;
           
           dct:hasVersion <http://dublincore.org/usage/terms/history/#issued-003> ;
           
           rdfs:isDefinedBy dct: .



###  http://purl.org/dc/terms/language

dct:language rdf:type owl:NamedIndividual ;
             
             rdfs:label "Language"@en ;
             
             dct:issued "2008-01-14"^^xsd:date ;
             
             dct:modified "2008-01-14"^^xsd:date ;
             
             rdfs:comment "A language of the resource."@en ;
             
             dct:description "Recommended best practice is to use a controlled vocabulary such as RFC 4646 [RFC4646]."@en ;
             
             dct:hasVersion <http://dublincore.org/usage/terms/history/#languageT-001> ;
             
             rdfs:isDefinedBy dct: .



###  http://purl.org/dc/terms/license

dct:license rdf:type owl:NamedIndividual ;
            
            rdfs:label "License"@en ;
            
            dct:issued "2004-06-14"^^xsd:date ;
            
            dct:modified "2008-01-14"^^xsd:date ;
            
            rdfs:comment "A legal document giving official permission to do something with the resource."@en ;
            
            dct:hasVersion <http://dublincore.org/usage/terms/history/#license-002> ;
            
            rdfs:isDefinedBy dct: .



###  http://purl.org/dc/terms/mediator

dct:mediator rdf:type owl:NamedIndividual ;
             
             rdfs:label "Mediator"@en ;
             
             dct:issued "2001-05-21"^^xsd:date ;
             
             dct:modified "2008-01-14"^^xsd:date ;
             
             rdfs:comment "An entity that mediates access to the resource and for whom the resource is intended or useful."@en ;
             
             dct:description "In an educational context, a mediator might be a parent, teacher, teaching assistant, or care-giver."@en ;
             
             dct:hasVersion <http://dublincore.org/usage/terms/history/#mediator-003> ;
             
             rdfs:isDefinedBy dct: .



###  http://purl.org/dc/terms/medium

dct:medium rdf:type owl:NamedIndividual ;
           
           rdfs:label "Medium"@en ;
           
           dct:issued "2000-07-11"^^xsd:date ;
           
           dct:modified "2008-01-14"^^xsd:date ;
           
           rdfs:comment "The material or physical carrier of the resource."@en ;
           
           dct:hasVersion <http://dublincore.org/usage/terms/history/#medium-003> ;
           
           rdfs:isDefinedBy dct: .



###  http://purl.org/dc/terms/modified

dct:modified rdf:type owl:DatatypeProperty ,
                      owl:NamedIndividual ;
             
             rdfs:label "Date Modified"@en ;
             
             dct:issued "2000-07-11"^^xsd:date ;
             
             dct:modified "2008-01-14"^^xsd:date ;
             
             rdfs:comment "Date on which the resource was changed."@en ;
             
             dct:hasVersion <http://dublincore.org/usage/terms/history/#modified-003> ;
             
             rdfs:isDefinedBy dct: .



###  http://purl.org/dc/terms/provenance

dct:provenance rdf:type owl:NamedIndividual ;
               
               rdfs:label "Provenance"@en ;
               
               dct:issued "2004-09-20"^^xsd:date ;
               
               dct:modified "2008-01-14"^^xsd:date ;
               
               rdfs:comment "A statement of any changes in ownership and custody of the resource since its creation that are significant for its authenticity, integrity, and interpretation."@en ;
               
               dct:description "The statement may include a description of any changes successive custodians made to the resource."@en ;
               
               dct:hasVersion <http://dublincore.org/usage/terms/history/#provenance-002> ;
               
               rdfs:isDefinedBy dct: .



###  http://purl.org/dc/terms/publisher

dct:publisher rdf:type owl:NamedIndividual ;
              
              rdfs:label "Publisher"@en ;
              
              dct:issued "2008-01-14"^^xsd:date ;
              
              dct:modified "2010-10-11"^^xsd:date ;
              
              rdfs:comment "An entity responsible for making the resource available."@en ;
              
              dct:description "Examples of a Publisher include a person, an organization, or a service."@en ;
              
              dct:hasVersion <http://dublincore.org/usage/terms/history/#publisherT-001> ;
              
              rdfs:isDefinedBy dct: .



###  http://purl.org/dc/terms/references

dct:references rdf:type owl:NamedIndividual ;
               
               rdfs:label "References"@en ;
               
               dct:issued "2000-07-11"^^xsd:date ;
               
               dct:modified "2008-01-14"^^xsd:date ;
               
               rdfs:comment "A related resource that is referenced, cited, or otherwise pointed to by the described resource."@en ;
               
               skos:note "This term is intended to be used with non-literal values as defined in the DCMI Abstract Model (http://dublincore.org/documents/abstract-model/).  As of December 2007, the DCMI Usage Board is seeking a way to express this intention with a formal range declaration."@en ;
               
               dct:hasVersion <http://dublincore.org/usage/terms/history/#references-003> ;
               
               rdfs:isDefinedBy dct: .



###  http://purl.org/dc/terms/relation

dct:relation rdf:type owl:NamedIndividual ;
             
             rdfs:label "Relation"@en ;
             
             dct:modified "2008-01-14"^^xsd:date ;
             
             dct:issued "2008-01-14"^^xsd:date ;
             
             rdfs:comment "A related resource."@en ;
             
             dct:description "Recommended best practice is to identify the related resource by means of a string conforming to a formal identification system. "@en ;
             
             skos:note "This term is intended to be used with non-literal values as defined in the DCMI Abstract Model (http://dublincore.org/documents/abstract-model/).  As of December 2007, the DCMI Usage Board is seeking a way to express this intention with a formal range declaration."@en ;
             
             dct:hasVersion <http://dublincore.org/usage/terms/history/#relationT-001> ;
             
             rdfs:isDefinedBy dct: .



###  http://purl.org/dc/terms/replaces

dct:replaces rdf:type owl:NamedIndividual ;
             
             rdfs:label "Replaces"@en ;
             
             dct:issued "2000-07-11"^^xsd:date ;
             
             dct:modified "2008-01-14"^^xsd:date ;
             
             rdfs:comment "A related resource that is supplanted, displaced, or superseded by the described resource."@en ;
             
             skos:note "This term is intended to be used with non-literal values as defined in the DCMI Abstract Model (http://dublincore.org/documents/abstract-model/).  As of December 2007, the DCMI Usage Board is seeking a way to express this intention with a formal range declaration."@en ;
             
             dct:hasVersion <http://dublincore.org/usage/terms/history/#replaces-003> ;
             
             rdfs:isDefinedBy dct: .



###  http://purl.org/dc/terms/requires

dct:requires rdf:type owl:NamedIndividual ;
             
             rdfs:label "Requires"@en ;
             
             dct:issued "2000-07-11"^^xsd:date ;
             
             dct:modified "2008-01-14"^^xsd:date ;
             
             rdfs:comment "A related resource that is required by the described resource to support its function, delivery, or coherence."@en ;
             
             skos:note "This term is intended to be used with non-literal values as defined in the DCMI Abstract Model (http://dublincore.org/documents/abstract-model/).  As of December 2007, the DCMI Usage Board is seeking a way to express this intention with a formal range declaration."@en ;
             
             dct:hasVersion <http://dublincore.org/usage/terms/history/#requires-003> ;
             
             rdfs:isDefinedBy dct: .



###  http://purl.org/dc/terms/rights

dct:rights rdf:type owl:NamedIndividual ;
           
           rdfs:label "Rights"@en ;
           
           dct:issued "2008-01-14"^^xsd:date ;
           
           dct:modified "2008-01-14"^^xsd:date ;
           
           rdfs:comment "Information about rights held in and over the resource."@en ;
           
           dct:description "Typically, rights information includes a statement about various property rights associated with the resource, including intellectual property rights."@en ;
           
           dct:hasVersion <http://dublincore.org/usage/terms/history/#rightsT-001> ;
           
           rdfs:isDefinedBy dct: .



###  http://purl.org/dc/terms/rightsHolder

dct:rightsHolder rdf:type owl:NamedIndividual ;
                 
                 rdfs:label "Rights Holder"@en ;
                 
                 dct:issued "2004-06-14"^^xsd:date ;
                 
                 dct:modified "2008-01-14"^^xsd:date ;
                 
                 rdfs:comment "A person or organization owning or managing rights over the resource."@en ;
                 
                 dct:hasVersion <http://dublincore.org/usage/terms/history/#rightsHolder-002> ;
                 
                 rdfs:isDefinedBy dct: .



###  http://purl.org/dc/terms/source

dct:source rdf:type owl:NamedIndividual ;
           
           rdfs:label "Source"@en ;
           
           dct:modified "2008-01-14"^^xsd:date ;
           
           dct:issued "2008-01-14"^^xsd:date ;
           
           rdfs:comment "A related resource from which the described resource is derived."@en ;
           
           dct:description "The described resource may be derived from the related resource in whole or in part. Recommended best practice is to identify the related resource by means of a string conforming to a formal identification system."@en ;
           
           skos:note "This term is intended to be used with non-literal values as defined in the DCMI Abstract Model (http://dublincore.org/documents/abstract-model/).  As of December 2007, the DCMI Usage Board is seeking a way to express this intention with a formal range declaration."@en ;
           
           dct:hasVersion <http://dublincore.org/usage/terms/history/#sourceT-001> ;
           
           rdfs:isDefinedBy dct: .



###  http://purl.org/dc/terms/spatial

dct:spatial rdf:type owl:NamedIndividual ;
            
            rdfs:label "Spatial Coverage"@en ;
            
            dct:issued "2000-07-11"^^xsd:date ;
            
            dct:modified "2008-01-14"^^xsd:date ;
            
            rdfs:comment "Spatial characteristics of the resource."@en ;
            
            dct:hasVersion <http://dublincore.org/usage/terms/history/#spatial-003> ;
            
            rdfs:isDefinedBy dct: .



###  http://purl.org/dc/terms/subject

dct:subject rdf:type owl:NamedIndividual ;
            
            rdfs:label "Subject"@en ;
            
            dct:issued "2008-01-14"^^xsd:date ;
            
            dct:modified "2012-06-14"^^xsd:date ;
            
            rdfs:comment "The topic of the resource."@en ;
            
            skos:note "This term is intended to be used with non-literal values as defined in the DCMI Abstract Model (http://dublincore.org/documents/abstract-model/).  As of December 2007, the DCMI Usage Board is seeking a way to express this intention with a formal range declaration."@en ;
            
            dct:description "Typically, the subject will be represented using keywords, key phrases, or classification codes. Recommended best practice is to use a controlled vocabulary."@en ;
            
            dct:hasVersion <http://dublincore.org/usage/terms/history/#subjectT-002> ;
            
            rdfs:isDefinedBy dct: .



###  http://purl.org/dc/terms/tableOfContents

dct:tableOfContents rdf:type owl:NamedIndividual ;
                    
                    rdfs:label "Table Of Contents"@en ;
                    
                    dct:issued "2000-07-11"^^xsd:date ;
                    
                    dct:modified "2008-01-14"^^xsd:date ;
                    
                    rdfs:comment "A list of subunits of the resource."@en ;
                    
                    dct:hasVersion <http://dublincore.org/usage/terms/history/#tableOfContents-003> ;
                    
                    rdfs:isDefinedBy dct: .



###  http://purl.org/dc/terms/temporal

dct:temporal rdf:type owl:NamedIndividual ;
             
             rdfs:label "Temporal Coverage"@en ;
             
             dct:issued "2000-07-11"^^xsd:date ;
             
             dct:modified "2008-01-14"^^xsd:date ;
             
             rdfs:comment "Temporal characteristics of the resource."@en ;
             
             dct:hasVersion <http://dublincore.org/usage/terms/history/#temporal-003> ;
             
             rdfs:isDefinedBy dct: .



###  http://purl.org/dc/terms/title

dct:title rdf:type owl:NamedIndividual ;
          
          rdfs:label "Title"@en ;
          
          dct:issued "2008-01-14"^^xsd:date ;
          
          dct:modified "2010-10-11"^^xsd:date ;
          
          rdfs:comment "A name given to the resource."@en ;
          
          dct:hasVersion <http://dublincore.org/usage/terms/history/#titleT-002> ;
          
          rdfs:isDefinedBy dct: .



###  http://purl.org/dc/terms/type

dct:type rdf:type owl:NamedIndividual ;
         
         rdfs:label "Type"@en ;
         
         dct:modified "2008-01-14"^^xsd:date ;
         
         dct:issued "2008-01-14"^^xsd:date ;
         
         dct:description "Recommended best practice is to use a controlled vocabulary such as the DCMI Type Vocabulary [DCMITYPE]. To describe the file format, physical medium, or dimensions of the resource, use the Format element."@en ;
         
         rdfs:comment "The nature or genre of the resource."@en ;
         
         dct:hasVersion <http://dublincore.org/usage/terms/history/#typeT-001> ;
         
         rdfs:isDefinedBy dct: .



###  http://purl.org/dc/terms/valid

dct:valid rdf:type owl:NamedIndividual ;
          
          rdfs:label "Date Valid"@en ;
          
          dct:issued "2000-07-11"^^xsd:date ;
          
          dct:modified "2008-01-14"^^xsd:date ;
          
          rdfs:comment "Date (often a range) of validity of a resource."@en ;
          
          dct:hasVersion <http://dublincore.org/usage/terms/history/#valid-003> ;
          
          rdfs:isDefinedBy dct: .




###  Generated by the OWL API (version 3.5.0) http://owlapi.sourceforge.net

